src/bva/BVList.v
@@ -115,6 +115,7 @@ Parameter size_bv_mult  : bitvector -> bitvector -> N.
 
 Axiom bits_size      : forall bv, List.length (bits bv) = N.to_nat (size bv).
 Axiom of_bits_size   : forall l, N.to_nat (size (of_bits l)) = List.length l.
+
 Axiom zeros_size     : forall n, size (zeros n) = n.
 Axiom bv_concat_size : forall n m a b, size a = n -> size b = m -> size (bv_concat a b) = n + m.
 Axiom bv_and_size    : forall a b, size (bv_and a b) = size_bv_and a b.
@@ -288,6 +289,2478 @@ Qed.
   (* Qed. *)
 
 End RAW2BITVECTOR.
+
+
+Module Type BITVECTOR_FIXED.
+
+  Parameter _size     : N.
+  
+  Parameter bitvector : Type.
+  Parameter bits      : bitvector -> list bool.
+  Parameter of_bits   : list bool -> bitvector.
+  Parameter bitOf     : nat -> bitvector -> bool.
+  Parameter size      : bitvector -> N.
+
+  (* Constants *)
+  Parameter zeros     : bitvector.
+
+  (*equality*)
+  Parameter bv_eq     : bitvector -> bitvector -> bool.
+
+  (*binary operations*)
+  (* Parameter bv_concat : forall n m, bitvector n -> bitvector m -> bitvector (n + m). *)
+  Parameter bv_and    : bitvector -> bitvector -> bitvector.
+  Parameter bv_or     : bitvector -> bitvector -> bitvector.
+  Parameter bv_xor    : bitvector -> bitvector -> bitvector.
+  Parameter bv_add    : bitvector -> bitvector -> bitvector.
+  Parameter bv_subst  : bitvector -> bitvector -> bitvector.
+
+  Parameter bv_mult   : bitvector -> bitvector -> bitvector.
+
+  (* forall (bv1 bv2 : bitvector), (size bv1 = size bv2) -> bitvector. *)
+  (* Parameter bv_xor    : forall n, bitvector n -> bitvector n -> bitvector n. *)
+  (* Parameter bv_add    : forall n, bitvector n -> bitvector n -> bitvector n. *)
+  (* Parameter bv_subst  : forall n, bitvector n -> bitvector n -> bitvector n. *)
+  (* Parameter bv_mult   : forall n, bitvector n -> bitvector n -> bitvector n. *)
+
+  (*binary operations*)
+  (* Parameter bv_not    : forall n, bitvector n -> bitvector n. *)
+
+  (* Specification *)
+  Axiom bits_size     : forall bv, _size = (size bv).
+
+(*  Axiom bits_size     : forall bv, N.of_nat (length (bits bv)) = (size bv). *)
+  
+  Axiom bv_eq_reflect : forall (a b:bitvector), bv_eq a b = true <-> a = b.
+  (* Axiom bv_and_comm   : forall n (a b:bitvector n), bv_eq (bv_and a b) (bv_and b a) = true. *)
+  (* Axiom bv_or_comm    : forall n (a b:bitvector n), bv_eq (bv_or a b) (bv_or b a) = true. *)
+  Axiom bv_add_comm   : forall (a b:bitvector), size a = _size -> size b = _size -> bv_eq (bv_add a b) (bv_add b a) = true.
+  (* Axiom bv_mult_comm  : forall n (a b:bitvector n), bv_eq (bv_mult a b) (bv_mult b a) = true.  *)
+
+  (* Axiom bv_and_assoc  : forall n (a b c: bitvector n), bv_eq (bv_and a (bv_and b c)) (bv_and (bv_and a b) c) = true. *)
+  (* Axiom bv_or_assoc   : forall n (a b c: bitvector n), bv_eq (bv_or a (bv_or b c)) (bv_or (bv_or a b) c) = true. *)
+  (* Axiom bv_xor_assoc  : forall n (a b c: bitvector n), bv_eq (bv_xor a (bv_xor b c)) (bv_xor (bv_xor a b) c) = true. *)
+  (* Axiom bv_add_assoc  : forall n (a b c: bitvector n), bv_eq (bv_add a (bv_add b c)) (bv_add (bv_add a b) c) = true. *)
+  (* Axiom bv_not_involutative: forall n (a: bitvector n), bv_eq (bv_not (bv_not a)) a = true. *)
+
+End BITVECTOR_FIXED.
+
+Module Type RAWBITVECTOR_FIXED.
+
+Parameter _size      : N.
+
+Parameter bitvector  : Type.
+Parameter size       : bitvector -> N.
+Parameter bits       : bitvector -> list bool.
+Parameter of_bits    : list bool -> bitvector.
+Parameter bitOf      : nat -> bitvector -> bool.
+
+(* Constants *)
+Parameter zeros      : bitvector.
+
+(*equality*)
+Parameter bv_eq      : bitvector -> bitvector -> bool.
+
+(*binary operations*)
+Parameter bv_concat  : bitvector -> bitvector -> bitvector.
+Parameter bv_and     : bitvector -> bitvector -> bitvector.
+Parameter bv_or      : bitvector -> bitvector -> bitvector.
+Parameter bv_xor     : bitvector -> bitvector -> bitvector.
+Parameter bv_add     : bitvector -> bitvector -> bitvector.
+Parameter bv_mult    : bitvector -> bitvector -> bitvector.
+Parameter bv_subst   : bitvector -> bitvector -> bitvector.
+
+(*unary operations*)
+Parameter bv_not     : bitvector -> bitvector.
+
+Parameter size_bv_and   : bitvector -> bitvector -> N.
+Parameter size_bv_or    : bitvector -> bitvector -> N.
+Parameter size_bv_xor   : bitvector -> bitvector -> N.
+Parameter size_bv_add   : bitvector -> bitvector -> N.
+Parameter size_bv_subst : bitvector -> bitvector -> N.
+Parameter size_bv_mult  : bitvector -> bitvector -> N.
+
+(* All the operations are size-preserving *)
+
+(* Axiom bits_size     : forall bv, N.of_nat (length (bits bv)) = (size bv). *)
+(* Axiom bits_size     : forall bv, _size = (size bv). *)
+
+(**)
+Axiom of_bits_size  : forall l, size (of_bits l) = _size.
+
+Axiom zeros_size     : size (zeros) = _size.
+(*Axiom bv_concat_size : forall n m a b, size a = n -> size b = m -> size (bv_concat a b) = n + m.*)
+Axiom bv_and_size    : forall a b, size (bv_and a b) = _size.
+Axiom bv_or_size     : forall a b, size (bv_or a b) = _size.
+Axiom bv_xor_size    : forall a b, size (bv_xor a b) = _size.
+Axiom bv_add_size    : forall a b, size (bv_add a b) = _size.
+Axiom bv_subst_size  : forall a b, size (bv_subst a b) = _size.
+Axiom bv_mult_size   : forall a b, size (bv_mult a b) = _size.
+
+(* Axiom bv_or_size     : forall a b, size a = size b -> size (bv_or a b) = size a. *)
+(* Axiom bv_xor_size    : forall a b, size a = n -> size b = n -> size (bv_xor a b) = n. *)
+(* Axiom bv_add_size    : forall a b, size a = n -> size b = n -> size (bv_add a b) = n. *)
+(* Axiom bv_subst_size  : forall a b, size a = n -> size b = n -> size (bv_subst a b) = n. *)
+(* Axiom bv_mult_size   : forall a b, size a = n -> size b = n -> size (bv_mult a b) = n. *)
+(* Axiom bv_not_size    : forall n a, size a = n -> size (bv_not a) = n. *)
+
+(* Specification *)
+ Axiom bv_eq_reflect  : forall a b, bv_eq a b = true <-> a = b.
+(*Axiom bv_eq_reflect  : forall a b, bv_eq a b = true <-> (size a = size b /\ a = b).*)
+Axiom bv_and_comm    : forall a b, size a = _size -> size b = _size -> bv_and a b = bv_and b a.
+Axiom bv_or_comm     : forall a b, size a = _size -> size b = _size -> bv_or a b = bv_or b a.
+Axiom bv_add_comm    : forall a b, size a = _size -> size b = _size -> bv_add a b = bv_add b a.
+(* Axiom bv_mult_comm   : forall n a b, size a = n -> size b = n -> bv_mult a b = bv_mult b a. *)
+
+Axiom bv_and_assoc  : forall a b c, size a = _size -> size b = _size -> size c = _size -> 
+                                   (bv_and a (bv_and b c)) = (bv_and (bv_and a b) c).
+Axiom bv_or_assoc   : forall a b c, size a = _size -> size b = _size -> size c = _size -> 
+                                   (bv_or a (bv_or b c)) = (bv_or (bv_or a b) c).
+Axiom bv_xor_assoc  : forall a b c, size a = _size -> size b = _size -> size c = _size -> 
+                                   (bv_xor a (bv_xor b c)) = (bv_xor (bv_xor a b) c).
+Axiom bv_add_assoc  : forall a b c, size a = _size -> size b = _size -> size c = _size -> 
+                                   (bv_add a (bv_add b c)) = (bv_add (bv_add a b) c).
+(*Axiom bv_not_involutative: forall a, bv_not (bv_not a) = a.*)
+
+End RAWBITVECTOR_FIXED.
+
+
+Module RAW2BITVECTOR_FIXED (M:RAWBITVECTOR_FIXED) <: BITVECTOR_FIXED.
+
+  Definition _size := M._size.
+ 
+  Record bitvector_  : Type :=
+    MkBitvector
+      { bv :> M.bitvector;
+        wf : M.size bv = _size
+      }.
+  Definition bitvector := bitvector_.
+
+  Definition bits (bv:bitvector) := M.bits bv.
+
+  Definition size (bv:bitvector) := M.size bv.
+
+  Lemma of_bits_size l : M.size (M.of_bits l) = _size.
+  Proof. rewrite M.of_bits_size. now unfold _size. Qed.
+
+  Definition of_bits (l:list bool) : bitvector  :=
+    @MkBitvector (M.of_bits l) (of_bits_size l).
+
+  Definition bitOf p (bv:bitvector) : bool := M.bitOf p bv.
+
+  Definition zeros : bitvector := 
+    @MkBitvector (M.zeros) (M.zeros_size).
+
+  Definition bv_eq (bv1 bv2:bitvector) := M.bv_eq bv1 bv2.
+
+  Definition bv_and (bv1 bv2:bitvector) : bitvector :=
+    @MkBitvector (M.bv_and bv1 bv2) (M.bv_and_size bv1 bv2).
+
+  Definition bv_or (bv1 bv2:bitvector) : bitvector :=
+    @MkBitvector (M.bv_or bv1 bv2) (M.bv_or_size bv1 bv2).
+
+  Definition bv_xor (bv1 bv2:bitvector) : bitvector :=
+    @MkBitvector (M.bv_xor bv1 bv2) (M.bv_xor_size bv1 bv2).
+
+  Definition bv_add (bv1 bv2:bitvector) : bitvector :=
+    @MkBitvector (M.bv_add bv1 bv2) (M.bv_add_size bv1 bv2).
+
+  Definition bv_subst (bv1 bv2:bitvector) : bitvector :=
+    @MkBitvector (M.bv_subst bv1 bv2) (M.bv_subst_size bv1 bv2).
+
+  Definition bv_mult (bv1 bv2:bitvector) : bitvector :=
+    @MkBitvector (M.bv_mult bv1 bv2) (M.bv_mult_size bv1 bv2).
+
+  (*  Definition bv_or (bv1 bv2:bitvector) (p: M.size bv1 = M.size bv2) : bitvector :=
+    @MkBitvector (M.bv_or bv1 bv2) (M.size bv1) (M.bv_or_size p). *)
+
+  (* Definition bv_add n (bv1 bv2:bitvector n) : bitvector n := *)
+  (*   @MkBitvector n (M.bv_add bv1 bv2) (M.bv_add_size (wf bv1) (wf bv2)). *)
+
+  (* Definition bv_subst n (bv1 bv2:bitvector n) : bitvector n := *)
+  (*   @MkBitvector n (M.bv_subst bv1 bv2) (M.bv_subst_size (wf bv1) (wf bv2)). *)
+
+  (* Definition bv_mult n (bv1 bv2:bitvector n) : bitvector n := *)
+  (*   @MkBitvector n (M.bv_mult bv1 bv2) (M.bv_mult_size (wf bv1) (wf bv2)). *)
+
+  (* Definition bv_xor n (bv1 bv2:bitvector n) : bitvector n := *)
+  (*   @MkBitvector n (M.bv_xor bv1 bv2) (M.bv_xor_size (wf bv1) (wf bv2)). *)
+
+  (* Definition bv_not n (bv1: bitvector n) : bitvector n := *)
+  (*   @MkBitvector n (M.bv_not bv1) (M.bv_not_size (wf bv1)). *)
+
+  (* Definition bv_concat n m (bv1:bitvector n) (bv2: bitvector m) : bitvector (n + m) := *)
+  (*   @MkBitvector (n + m) (M.bv_concat bv1 bv2) (M.bv_concat_size (wf bv1) (wf bv2)). *)
+
+
+(*
+  Lemma bits_size: forall bv, N.of_nat (length (bits bv)) = (size bv).
+  Proof. intros. unfold size, bits. rewrite M.bits_size.
+         destruct bv0. simpl. exact wf0.
+  Qed.
+*)
+
+ Lemma bits_size: forall bv, _size = (size bv).
+ Proof. intros. unfold size. destruct bv0. simpl. easy. Qed.
+
+
+Lemma bv_eq_reflect (a b: bitvector): bv_eq a b = true <-> a = b.
+Proof.
+    unfold bv_eq. rewrite M.bv_eq_reflect. split.
+
+    - revert a b.
+      intros [a Ha] [b Hb]. simpl.
+      intro. revert Ha Hb. rewrite H.
+      intros. specialize ( proof_irrelevance Ha Hb). intros.
+      now rewrite H0.
+
+    - intros. now destruct H.
+Qed.
+
+  Lemma bv_add_comm (a b:bitvector) :  size a = _size -> size b = _size -> bv_eq (bv_add a b) (bv_add b a) = true. 
+  Proof.
+    intros.
+    unfold bv_eq. rewrite M.bv_eq_reflect. apply (@M.bv_add_comm a b). 
+    destruct a. simpl. easy.
+    destruct b. simpl. easy.
+  Qed. 
+
+  (* Lemma bv_or_comm n (a b:bitvector n) : bv_eq (bv_or a b) (bv_or b a) = true. *)
+  (* Proof. *)
+  (*   unfold bv_eq. rewrite M.bv_eq_reflect. apply (@M.bv_or_comm n); now rewrite wf. *)
+  (* Qed. *)
+
+  (* Lemma bv_add_comm n (a b:bitvector n) : bv_eq (bv_add a b) (bv_add b a) = true. *)
+  (* Proof. *)
+  (*   unfold bv_eq. rewrite M.bv_eq_reflect. apply (@M.bv_add_comm n); now rewrite wf. *)
+  (* Qed. *)
+
+  (* Lemma bv_mult_comm n (a b:bitvector n) : bv_eq (bv_mult a b) (bv_mult b a) = true. *)
+  (* Proof. *)
+  (*   unfold bv_eq. rewrite M.bv_eq_reflect. apply (@M.bv_mult_comm n); now rewrite wf. *)
+  (* Qed. *)
+
+  (* Lemma bv_and_assoc : forall n (a b c :bitvector n), bv_eq (bv_and a (bv_and b c)) (bv_and (bv_and a b) c) = true. *)
+  (* Proof. *)
+  (*    intros n a b c. *)
+  (*    unfold bv_eq. rewrite M.bv_eq_reflect. simpl.  *)
+  (*    apply (@M.bv_and_assoc n a b c); now rewrite wf. *)
+  (* Qed. *)
+
+  (* Lemma bv_or_assoc : forall n (a b c :bitvector n), bv_eq (bv_or a (bv_or b c)) (bv_or (bv_or a b) c) = true. *)
+  (* Proof. *)
+  (*    intros n a b c. *)
+  (*    unfold bv_eq. rewrite M.bv_eq_reflect. simpl.  *)
+  (*    apply (@M.bv_or_assoc n a b c); now rewrite wf. *)
+  (* Qed. *)
+
+  (* Lemma bv_xor_assoc : forall n (a b c :bitvector n), bv_eq (bv_xor a (bv_xor b c)) (bv_xor (bv_xor a b) c) = true. *)
+  (* Proof. *)
+  (*    intros n a b c. *)
+  (*    unfold bv_eq. rewrite M.bv_eq_reflect. simpl.  *)
+  (*    apply (@M.bv_xor_assoc n a b c); now rewrite wf. *)
+  (* Qed. *)
+
+  (* Lemma bv_add_assoc : forall n (a b c :bitvector n), bv_eq (bv_add a (bv_add b c)) (bv_add (bv_add a b) c) = true. *)
+  (* Proof. *)
+  (*    intros n a b c. *)
+  (*    unfold bv_eq. rewrite M.bv_eq_reflect. simpl.  *)
+  (*    apply (@M.bv_add_assoc n a b c); now rewrite wf. *)
+  (* Qed. *)
+
+  (* Lemma bv_not_involutative: forall n (a: bitvector n), bv_eq (bv_not (bv_not a)) a = true. *)
+  (* Proof. *)
+  (*      intros n a. *)
+  (*      unfold bv_eq. rewrite M.bv_eq_reflect. simpl.  *)
+  (*      apply (@M.bv_not_involutative a); now rewrite wf. *)
+  (* Qed. *)
+
+End RAW2BITVECTOR_FIXED.
+
+
+
+Module RAWBITVECTOR_LIST_FIXED <: RAWBITVECTOR_FIXED.
+
+Variable _size: N.
+
+Definition bitvector := list bool.
+Definition bits (a:bitvector) : list bool := a.
+Definition size (a:bitvector) := N.of_nat (length a).
+
+
+Fixpoint mk_list_false (t: nat) : list bool :=
+  match t with
+    | O    => []
+    | S t' => false::(mk_list_false t')
+  end.
+
+Definition zeros : bitvector := mk_list_false (N.to_nat _size).
+
+Definition zero_len (n: N):  bitvector := mk_list_false (N.to_nat n).
+
+Definition of_bits (a:list bool) : bitvector := 
+if (N.eqb (N.of_nat (length a)) _size ) then a else zeros.
+
+Definition of_bits_len (a:list bool) (n: N) : bitvector := 
+if (N.eqb (N.of_nat (length a)) n ) then a else zero_len n.
+
+(*
+
+Lemma bits_size: forall bv, _size = N.of_nat (size bv).
+Proof. intros. now unfold size. Qed.
+*)
+
+Lemma length_mk_list_false: forall n, length (mk_list_false n) = n.
+Proof. intro n.
+       induction n as [ | n' IHn].
+       - simpl. auto.
+       - simpl. apply f_equal. exact IHn.
+Qed.
+
+Lemma zeros_size : size (zeros) = _size.
+Proof. unfold size, zeros. now rewrite length_mk_list_false, N2Nat.id. Qed. 
+
+Lemma zeros_len_size (n: N) : size (zero_len n) = n.
+Proof. unfold zero_len, size. now rewrite length_mk_list_false, N2Nat.id. Qed. 
+
+Lemma of_bits_size l: (size (of_bits l)) = _size.
+Proof. unfold of_bits.
+       case_eq (N.of_nat (length l) =? _size). intros.
+       now rewrite N.eqb_eq in H.
+       intros.
+       now rewrite zeros_size.
+Qed.
+
+Lemma of_bits_len_size (n: N) l: (size (of_bits_len l n)) = n.
+Proof. unfold of_bits_len.
+       case_eq (N.of_nat (length l) =? n). intros.
+       now rewrite N.eqb_eq in H.
+       intros.
+       now rewrite zeros_len_size.
+Qed.
+
+Definition beq_list (l m : list bool) := forallb2 Bool.eqb l m.
+
+Definition bv_eq (a b: bitvector): bool:=
+  beq_list (bits a) (bits b).
+
+Lemma bv_mk_eq l1 l2 : bv_eq l1 l2 = beq_list l1 l2.
+Proof.
+  unfold bv_eq, size, bits. reflexivity.
+Qed.
+
+Definition bv_concat (a b: bitvector) : bitvector := a ++ b.
+
+Section Map2.
+
+  Variables A B C: Type.
+  Variable f : A -> B -> C.
+
+  Fixpoint map2 (l1 : list A) (l2 : list B) {struct l1} : list C :=
+    match l1, l2 with
+      | b1::tl1, b2::tl2 => (f b1 b2)::(map2 tl1 tl2)
+      | _, _ => nil
+    end.
+
+End Map2.
+
+Section Fold_left2.
+
+  Variables A B: Type.
+  Variable f : A -> B -> B -> A.
+
+  Fixpoint fold_left2 (xs ys: list B) (acc:A) {struct xs} : A :=
+    match xs, ys with
+    | nil, _ | _, nil => acc
+    | x::xs, y::ys    => fold_left2 xs ys (f acc x y)
+    end.
+
+  Lemma foo : forall (I: A -> Prop) acc, I acc -> 
+              (forall a b1 b2, I a -> I (f a b1 b2)) -> 
+              forall xs ys, I (fold_left2 xs ys acc).
+  Proof. intros I acc H0 H1 xs. revert acc H0.
+         induction xs as [ | a xs IHxs]; intros acc H.
+         simpl. auto.
+         intros [ | b ys].
+            + simpl. exact H.
+            + simpl. apply IHxs, H1. exact H.
+  Qed.
+
+
+End Fold_left2.
+
+Definition bitOf (n: nat) (a: bitvector): bool := nth n a false.
+
+Definition bv_and (a b : bitvector) : bitvector :=
+  if ((@size a) =? _size) && ((@size b) =? _size)
+  then map2 andb (@bits a) (@bits b)
+  else zeros.
+
+Definition bv_or (a b : bitvector) : bitvector :=
+  if ((@size a) =? _size) && ((@size b) =? _size)
+  then map2 orb (@bits a) (@bits b)
+  else zeros.
+
+Definition bv_xor (a b : bitvector) : bitvector :=
+  if ((@size a) =? _size) && ((@size b) =? _size)
+  then map2 xorb (@bits a) (@bits b)
+  else zeros.
+
+Definition bv_not (a: bitvector) : bitvector := map negb (@bits a).
+
+(*arithmetic operations*)
+
+ (*addition*)
+
+Definition add_carry b1 b2 c :=
+  match b1, b2, c with
+    | true,  true,  true  => (true, true)
+    | true,  true,  false
+    | true,  false, true
+    | false, true,  true  => (false, true)
+    | false, false, true
+    | false, true,  false
+    | true,  false, false => (true, false)
+    | false, false, false => (false, false)
+  end.
+
+(* Truncating addition in little-endian, direct style *)
+
+Fixpoint add_list_ingr bs1 bs2 c {struct bs1} :=
+  match bs1, bs2 with
+    | nil, _               => nil
+    | _ , nil              => nil
+    | b1 :: bs1, b2 :: bs2 =>
+      let (r, c) := add_carry b1 b2 c in r :: (add_list_ingr bs1 bs2 c)
+  end.
+
+Definition add_list (a b: list bool) := add_list_ingr a b false.
+
+Definition bv_add (a b : bitvector) : bitvector :=
+  if ((@size a) =? _size) && ((@size b) =? _size)
+  then add_list a b
+  else zeros.
+
+  (*substraction*)
+
+Definition twos_complement b :=
+  add_list_ingr (map negb b) (mk_list_false (length b)) true.
+
+Definition subst_list' a b := add_list a (twos_complement b).
+
+Definition bv_subst' (a b : bitvector) : bitvector :=
+   match (@size a) =? (@size b) with
+     | true => (subst_list' (@bits a) (@bits b))
+     | _    => zeros
+   end.
+
+Definition subst_borrow b1 b2 b :=
+  match b1, b2, b with
+    | true,  true,  true  => (true, true)
+    | true,  true,  false => (false, false)
+    | true,  false, true  => (false, false)
+    | false, true,  true  => (false, true)
+    | false, false, true  => (true, true)
+    | false, true,  false => (true, true)
+    | true,  false, false => (true, false)
+    | false, false, false => (false, false)
+  end.
+
+Fixpoint subst_list_borrow bs1 bs2 b {struct bs1} :=
+  match bs1, bs2 with
+    | nil, _               => nil
+    | _ , nil              => nil
+    | b1 :: bs1, b2 :: bs2 =>
+      let (r, b) := subst_borrow b1 b2 b in r :: (subst_list_borrow bs1 bs2 b)
+  end.
+
+Definition subst_list (a b: list bool) := subst_list_borrow a b false.
+
+Definition bv_subst (a b : bitvector) : bitvector :=
+  if ((@size a) =? _size) && ((@size b) =? _size)
+  then subst_list a b
+  else zeros.
+  (*multiplication*)
+
+Fixpoint mult_list_carry (a b :list bool) n {struct a}: list bool :=
+  match a with
+    | nil      => mk_list_false n
+    | a' :: xs =>
+      if a' then
+        add_list b (mult_list_carry xs (false :: b) n)
+      else
+        mult_list_carry xs (false :: b) n
+  end.
+
+Fixpoint mult_list_carry2 (a b :list bool) n {struct a}: list bool :=
+  match a with
+    | nil      => mk_list_false n
+    | a' :: xs =>
+      if a' then
+        add_list b (mult_list_carry2 xs (false :: (removelast b)) n)
+      else
+        mult_list_carry2 xs (false :: (removelast b)) n
+  end.
+
+
+Fixpoint and_with_bool (a: list bool) (bt: bool) : list bool :=
+  match a with
+    | nil => nil
+    | ai :: a' => (bt && ai) :: and_with_bool a' bt 
+  end.
+
+
+Fixpoint mult_bool_step_k_h (a b: list bool) (c: bool) (k: Z) : list bool :=
+  match a, b with
+    | nil , _ => nil
+    | ai :: a', bi :: b' =>
+      if (k - 1 <? 0)%Z then
+        let carry_out := (ai && bi) || ((xorb ai bi) && c) in
+        let curr := xorb (xorb ai bi) c in
+        curr :: mult_bool_step_k_h a' b' carry_out (k - 1)
+      else
+        ai :: mult_bool_step_k_h a' b c (k - 1)
+    | ai :: a' , nil => ai :: mult_bool_step_k_h a' b c k
+  end.
+
+
+Fixpoint top_k_bools (a: list bool) (k: int) : list bool :=
+  if (k == 0)%int63 then nil
+  else match a with
+         | nil => nil
+         | ai :: a' => ai :: top_k_bools a' (k - 1)
+       end.
+
+
+Fixpoint mult_bool_step (a b: list bool) (res: list bool) (k k': nat) : list bool :=
+  let ak := List.firstn (S k') a in
+  let b' := and_with_bool ak (nth k b false) in
+  let res' := mult_bool_step_k_h res b' false (Z.of_nat k) in
+  match k' with
+    | O => res'
+    (* | S O => res' *)
+    | S pk' => mult_bool_step a b res' (S k) pk'
+  end.
+
+
+Definition bvmult_bool (a b: list bool) (n: nat) : list bool :=
+  let res := and_with_bool a (nth 0 b false) in
+  match n with
+    | O => res
+    | S O => res
+    | S (S k) => mult_bool_step a b res 1 k
+  end.
+
+(*
+Definition check_mult_bool (bs1 bs2 bsres: list bool) : bool :=
+    let bvm12 := bvmult_bool bs1 bs2 (length bsres) in
+    forallb2 eq_carry_lit bvm12 bsres.
+
+
+Lemma prop_main: forall bs1 bs2 bsres,
+                 check_mult bs1 bs2 bsres = true ->
+                 (bvmult_bool bs1 bs2 (length bs1)) = bsres.
+*)
+
+Definition mult_list a b := bvmult_bool a b (length a).
+
+Definition bv_mult (a b : bitvector) : bitvector :=
+  if ((@size a) =? _size) && ((@size b) =? _size)
+  then mult_list a b
+  else zeros.
+
+
+(* Theorems *)
+
+(*
+Lemma length_mk_list_true: forall n, length (mk_list_true n) = n.
+Proof. intro n.
+       induction n as [ | n' IHn].
+       - simpl. auto.
+       - simpl. apply f_equal. exact IHn.
+Qed.
+*)
+
+Lemma List_eq : forall (l m: list bool), beq_list l m = true <-> l = m.
+Proof.
+    induction l; destruct m; simpl; split; intro; try (reflexivity || discriminate).
+    - rewrite andb_true_iff in H. destruct H. rewrite eqb_true_iff in H. rewrite H.
+    apply f_equal. apply IHl. exact H0.
+    - inversion H. subst b. subst m. rewrite andb_true_iff. split.
+      + apply eqb_reflx.
+      + apply IHl; reflexivity.
+Qed.
+
+Lemma List_eq_refl : forall (l m: list bool), beq_list l l = true.
+Proof.
+    induction l; simpl; intro; try (reflexivity || discriminate).
+    - rewrite andb_true_iff. split. apply eqb_reflx. apply IHl. exact m.
+Qed.
+
+Lemma bv_eq_reflect a b : bv_eq a b = true <-> a = b.
+Proof.
+  unfold bv_eq. unfold bits. apply List_eq.
+Qed.
+
+(*
+Lemma bv_concat_size n m a b : size a = n -> size b = m -> size (bv_concat a b) = n + m.
+Proof.
+  unfold bv_concat, size. intros H0 H1.
+  rewrite app_length, Nat2N.inj_add, H0, H1; reflexivity.
+Qed.
+
+*)
+
+(*list bitwise AND properties*)
+
+Lemma map2_and_comm: forall (a b: list bool), (map2 andb a b) = (map2 andb b a).
+Proof. intros a. induction a as [ | a' xs IHxs].
+       intros [ | b' ys].
+       - simpl. auto.
+       - simpl. auto.
+       - intros [ | b' ys].
+         + simpl. auto.
+         + intros. simpl. 
+           cut (a' && b' = b' && a'). intro H. rewrite <- H. apply f_equal.
+           apply IHxs. apply andb_comm.
+Qed.
+
+Lemma map2_and_assoc: forall (a b c: list bool), (map2 andb a (map2 andb b c)) = (map2 andb (map2 andb a b) c).
+Proof. intro a. induction a as [ | a' xs IHxs].
+       simpl. auto.
+       intros [ | b' ys].
+        -  simpl. auto.
+        - intros [ | c' zs].
+          + simpl. auto.
+          + simpl. cut (a' && (b' && c') = a' && b' && c'). intro H. rewrite <- H. apply f_equal.
+            apply IHxs. apply andb_assoc.
+Qed.
+
+Lemma map2_and_idem1:  forall (a b: list bool), (map2 andb (map2 andb a b) a) = (map2 andb a b).
+Proof. intros a. induction a as [ | a' xs IHxs].
+       intros [ | b' ys].
+       - simpl. auto.
+       - simpl. auto.
+       - intros [ | b' ys].
+         + simpl. auto.
+         + intros. simpl. 
+           cut (a' && b' && a' = a' && b'). intro H. rewrite H. apply f_equal.
+           apply IHxs. rewrite andb_comm, andb_assoc, andb_diag. reflexivity. 
+Qed.
+
+Lemma map2_and_idem_comm:  forall (a b: list bool), (map2 andb (map2 andb a b) a) = (map2 andb b a).
+Proof. intros a b. symmetry. rewrite <- map2_and_comm. symmetry; apply map2_and_idem1. Qed.
+
+Lemma map2_and_idem2:  forall (a b: list bool), (map2 andb (map2 andb a b) b) = (map2 andb a b).
+Proof. intros a. induction a as [ | a' xs IHxs].
+       intros [ | b' ys].
+       - simpl. auto.
+       - simpl. auto.
+       - intros [ | b' ys].
+         + simpl. auto.
+         + intros. simpl. 
+           cut (a' && b' && b' = a' && b'). intro H. rewrite H. apply f_equal.
+           apply IHxs. rewrite <- andb_assoc. rewrite andb_diag. reflexivity. 
+Qed.
+
+Lemma map2_and_idem_comm2:  forall (a b: list bool), (map2 andb (map2 andb a b) b) = (map2 andb b a).
+Proof. intros a b. symmetry. rewrite <- map2_and_comm. symmetry; apply map2_and_idem2. Qed.
+
+Lemma map2_and_empty_empty1:  forall (a: list bool), (map2 andb a []) = [].
+Proof. intros a. induction a as [ | a' xs IHxs]; simpl; auto. Qed.
+
+Lemma map2_and_empty_empty2:  forall (a: list bool), (map2 andb [] a) = [].
+Proof. intros a. rewrite map2_and_comm. apply map2_and_empty_empty1. Qed.
+
+Lemma map2_nth_empty_false:  forall (i: nat), nth i [] false = false.
+Proof. intros i. induction i as [ | IHi]; simpl; reflexivity. Qed.
+
+(* Lemma mk_list_true_rev: forall n, (rev (mk_list_true n)) = mk_list_true n. *)
+
+(*
+Lemma mk_list_true_equiv: forall t acc, mk_list_true_acc t acc = (List.rev (mk_list_true t)) ++ acc.
+Proof. induction t as [ |t IHt]; auto; intro acc; simpl; rewrite IHt.
+       rewrite app_assoc_reverse.
+       apply f_equal. simpl. reflexivity.
+Qed.
+
+Lemma mk_list_false_equiv: forall t acc, mk_list_false_acc t acc = (List.rev (mk_list_false t)) ++ acc.
+Proof. induction t as [ |t IHt]; auto; intro acc; simpl; rewrite IHt. 
+       rewrite app_assoc_reverse.
+       apply f_equal. simpl. reflexivity.
+Qed.
+
+Lemma len_mk_list_true_empty: length (mk_list_true_acc 0 []) = 0%nat.
+Proof. simpl. reflexivity. Qed.
+
+Lemma add_mk_list_true: forall n acc, length (mk_list_true_acc n acc) = (n + length acc)%nat.
+Proof. intros n.
+       induction n as [ | n' IHn].
+         + auto.
+         + intro acc. simpl. rewrite IHn. simpl. lia.
+Qed.
+
+*)
+
+Lemma map2_and_nth_bitOf: forall (a b: list bool) (i: nat), 
+                          length a = length b ->
+                          (i <= (length a))%nat ->
+                          nth i (map2 andb a b) false = (nth i a false) && (nth i b false).
+Proof. intro a.
+       induction a as [ | a xs IHxs].
+         - intros [ | b ys].
+           + intros i H0 H1. do 2 rewrite map2_nth_empty_false. reflexivity.
+           + intros i H0 H1. rewrite map2_and_empty_empty2.
+             rewrite map2_nth_empty_false. reflexivity.
+         - intros [ | b ys].
+           + intros i H0 H1. rewrite map2_and_empty_empty1.
+             rewrite map2_nth_empty_false. rewrite andb_false_r. reflexivity.
+           + intros i H0 H1. simpl.
+             revert i H1. intros [ | i IHi].
+             * simpl. auto.
+             *   apply IHxs.
+                 inversion H0. reflexivity.
+                 inversion IHi; lia.
+Qed.
+
+(*
+Lemma length_mk_list_true_full: forall n, length (mk_list_true_acc n []) = n.
+Proof. intro n. rewrite (@add_mk_list_true n []). auto. Qed.
+
+Lemma mk_list_app: forall n acc, mk_list_true_acc n acc = mk_list_true_acc n [] ++ acc.
+Proof. intro n.
+       induction n as [ | n IHn].
+         + auto.
+         + intro acc. simpl in *. rewrite IHn. 
+           cut (mk_list_true_acc n [] ++ [true] = mk_list_true_acc n [true]). intro H.
+           rewrite <- H. rewrite <- app_assoc. unfold app. reflexivity.
+           rewrite <- IHn. reflexivity.
+Qed.
+
+Lemma mk_list_ltrue: forall n, mk_list_true_acc n [true] = mk_list_true_acc (S n) [].
+Proof. intro n. induction n as [ | n IHn]; auto. Qed.
+
+Lemma map2_and_1_neutral: forall (a: list bool), (map2 andb a (mk_list_true (length a))) = a.
+Proof. intro a.
+       induction a as [ | a xs IHxs]. 
+         + auto.
+         + simpl. rewrite IHxs.
+           rewrite andb_true_r. reflexivity.
+Qed.
+
+Lemma map2_and_0_absorb: forall (a: list bool), (map2 andb a (mk_list_false (length a))) = (mk_list_false (length a)).
+Proof. intro a. induction a as [ | a' xs IHxs].
+       - simpl. reflexivity.
+       - simpl. rewrite IHxs.
+         rewrite andb_false_r; reflexivity.
+Qed.
+
+*)
+Lemma map2_and_length: forall (a b: list bool), length a = length b -> length a = length (map2 andb a b).
+Proof. induction a as [ | a' xs IHxs].
+       simpl. auto.
+       intros [ | b ys].
+       - simpl. intros. exact H.
+       - intros. simpl in *. apply f_equal. apply IHxs.
+         inversion H; auto.
+Qed.
+
+(*bitvector AND properties*)
+
+
+Definition size_bv_and (a b: bitvector) := _size.
+(*
+    match (@size a) =? (@size b) with 
+    | true => (@size a)
+    | _    => 0%N
+  end.
+*)
+
+Lemma bv_and_size a b : size (bv_and a b) = _size.
+Proof.
+  unfold bv_and.
+  case_eq ((size a =? _size) && (size b =? _size)). intro same.
+  rewrite andb_true_iff in same.
+  destruct same.
+  rewrite N.eqb_eq in H, H0.
+  unfold bits, size in *.
+  rewrite <- map2_and_length. now rewrite H.
+  apply (f_equal (N.to_nat)) in H.
+  apply (f_equal (N.to_nat)) in H0.
+  rewrite Nat2N.id in H, H0.
+  now rewrite H, H0.
+  
+  intros. now rewrite zeros_size.
+Qed.
+
+
+Lemma bv_and_comm a b : size a = _size -> size b = _size -> bv_and a b = bv_and b a.
+(* Lemma bv_and_comm: forall a b, (size a) = (size b) -> bv_and a b = bv_and b a. *)
+Proof.
+  intros H1 H2. unfold bv_and. rewrite H1, H2.
+  rewrite N.eqb_compare, N.compare_refl.
+  rewrite map2_and_comm. reflexivity.
+Qed.
+
+Lemma bv_and_assoc: forall a b c, size a = _size -> size b = _size -> size c = _size -> 
+                                  (bv_and a (bv_and b c)) = (bv_and (bv_and a b) c).
+Proof. intros a b c H0 H1 H2.
+       unfold bv_and, bits, size in *. rewrite H0, H1, H2.  
+       rewrite N.eqb_compare. rewrite N.compare_refl.
+       rewrite andb_true_l. do 2 rewrite andb_true_r.
+       rewrite <- map2_and_length. rewrite H1.
+       rewrite <- map2_and_length. rewrite H0.
+       now rewrite <- map2_and_assoc.
+       
+       apply (f_equal (N.to_nat)) in H0.
+       apply (f_equal (N.to_nat)) in H1.
+       rewrite Nat2N.id in H0, H1.
+       now rewrite H0, H1.
+       
+       apply (f_equal (N.to_nat)) in H1.
+       apply (f_equal (N.to_nat)) in H2.
+       rewrite Nat2N.id in H1, H2.
+       now rewrite H1, H2. 
+Qed.
+
+(*
+Lemma bv_and_idem1:  forall a b, size a = _size -> size b = _size -> (bv_and (bv_and a b) a) = (bv_and a b).
+Proof. intros a b H0 H1.
+       unfold bv_and. rewrite H0. do 2 rewrite N.eqb_compare.
+       unfold size, bits in *.
+       rewrite N.compare_refl.
+       rewrite map2_and_idem1; reflexivity.
+Qed.
+
+Lemma bv_and_idem2: forall a b, size a = _size ->  size b = _size -> (bv_and (bv_and a b) b) = (bv_and a b).
+Proof. intros a b H0 H1.
+       unfold bv_and. rewrite H0. do 2 rewrite N.eqb_compare.
+       unfold size, bits in *.
+       rewrite N.compare_refl.
+       rewrite map2_and_idem2; reflexivity.
+Qed.
+*)
+
+Definition bv_empty: bitvector := nil.
+
+(*
+
+Lemma bv_and_empty_empty1: forall a, (bv_and a bv_empty) = bv_empty.
+Proof. intros a. unfold bv_empty, bv_and, size, bits. simpl.
+       rewrite map2_and_empty_empty1.
+       case_eq (N.compare (N.of_nat (length a)) 0); intro H; simpl.
+         - apply (N.compare_eq (N.of_nat (length a))) in H.
+           rewrite N.eqb_compare. now rewrite N.compare_refl.
+         - rewrite N.eqb_compare. now rewrite N.compare_refl.
+         - rewrite N.eqb_compare. now rewrite N.compare_refl.
+Qed.
+
+
+Lemma bv_and_nth_bitOf: forall a b (i: nat), 
+                          (size a) = _size -> (size b) = _size ->
+                          (i <= (nat_of_N (size a)))%nat ->
+                          nth i (bits (bv_and a b)) false = (nth i (bits a) false) && (nth i (bits b) false).
+Proof. intros a b i H0 H1 H2. 
+       unfold bv_and. rewrite H0, H1. rewrite N.eqb_compare. rewrite N.compare_refl.
+       apply map2_and_nth_bitOf; unfold size in *; unfold bits.
+       now rewrite <- Nat2N.inj_iff, H1. rewrite Nat2N.id in H2; exact H2.
+Qed.
+
+
+Lemma bv_and_empty_empty2: forall a, (bv_and bv_empty a) = bv_empty.
+Proof. intro a. unfold bv_and, bv_empty, size.
+       rewrite N.eqb_compare, N.compare_refl; easy.
+Qed.
+
+Lemma bv_and_1_neutral: forall a, (bv_and a (mk_list_true (length (bits a)))) = a.
+Proof. intro a. unfold bv_and.
+       rewrite N.eqb_compare. unfold size, bits.
+       rewrite N.compare_refl.
+       rewrite map2_and_1_neutral. reflexivity.
+Qed.
+
+Lemma bv_and_0_absorb: forall a, (bv_and a (mk_list_false (length (bits a)))) = (mk_list_false (length (bits a))).
+Proof. intro a. unfold bv_and.
+       rewrite N.eqb_compare. unfold size, bits. 
+       rewrite N.compare_refl.
+       rewrite map2_and_0_absorb. reflexivity.
+Qed.
+
+*)
+
+(* lists bitwise OR properties *)
+
+
+Definition size_bv_or (a b: bitvector) := _size.
+
+Lemma map2_or_comm: forall (a b: list bool), (map2 orb a b) = (map2 orb b a).
+Proof. intros a. induction a as [ | a' xs IHxs].
+       intros [ | b' ys].
+       - simpl. auto.
+       - simpl. auto.
+       - intros [ | b' ys].
+         + simpl. auto.
+         + intros. simpl. 
+           cut (a' || b' = b' || a'). intro H. rewrite <- H. apply f_equal.
+           apply IHxs. apply orb_comm.
+Qed.
+
+Lemma map2_or_assoc: forall (a b c: list bool), (map2 orb a (map2 orb b c)) = (map2 orb (map2 orb a b) c).
+Proof. intro a. induction a as [ | a' xs IHxs].
+       simpl. auto.
+       intros [ | b' ys].
+        -  simpl. auto.
+        - intros [ | c' zs].
+          + simpl. auto.
+          + simpl. cut (a' || (b' || c') = a' || b' || c'). intro H. rewrite <- H. apply f_equal.
+            apply IHxs. apply orb_assoc.
+Qed.
+
+Lemma map2_or_length: forall (a b: list bool), length a = length b -> length a = length (map2 orb a b).
+Proof. induction a as [ | a' xs IHxs].
+       simpl. auto.
+       intros [ | b ys].
+       - simpl. intros. exact H.
+       - intros. simpl in *. apply f_equal. apply IHxs.
+         inversion H; auto.
+Qed.
+
+Lemma map2_or_empty_empty1:  forall (a: list bool), (map2 orb a []) = [].
+Proof. intros a. induction a as [ | a' xs IHxs]; simpl; auto. Qed.
+
+Lemma map2_or_empty_empty2:  forall (a: list bool), (map2 orb [] a) = [].
+Proof. intros a. rewrite map2_or_comm. apply map2_or_empty_empty1. Qed.
+
+Lemma map2_or_nth_bitOf: forall (a b: list bool) (i: nat), 
+                          (length a) = (length b) ->
+                          (i <= (length a))%nat ->
+                          nth i (map2 orb a b) false = (nth i a false) || (nth i b false).
+Proof. intro a.
+       induction a as [ | a xs IHxs].
+         - intros [ | b ys].
+           + intros i H0 H1. do 2 rewrite map2_nth_empty_false. reflexivity.
+           + intros i H0 H1. rewrite map2_or_empty_empty2.
+             rewrite map2_nth_empty_false. contradict H1. simpl. unfold not. intros. easy.
+         - intros [ | b ys].
+           + intros i H0 H1. rewrite map2_or_empty_empty1.
+             rewrite map2_nth_empty_false. rewrite orb_false_r. rewrite H0 in H1.
+             contradict H1. simpl. unfold not. intros. easy.
+           + intros i H0 H1. simpl.
+             revert i H1. intros [ | i IHi].
+             * simpl. auto.
+             * apply IHxs.
+                 inversion H0; reflexivity.
+                 inversion IHi; lia.
+Qed.
+
+Lemma map2_or_0_neutral: forall (a: list bool), (map2 orb a (mk_list_false (length a))) = a.
+Proof. intro a.
+       induction a as [ | a xs IHxs]. 
+         + auto.
+         + simpl. rewrite IHxs.
+           rewrite orb_false_r. reflexivity.
+Qed.
+
+(*bitvector OR properties*)
+
+Lemma bv_or_size a b: size (bv_or a b) = _size.
+Admitted.
+(*
+Proof.
+  unfold bv_or.
+  case_eq (size a =? size b); intros.
+  - rewrite N.eqb_eq in H. now unfold size in *.
+  - unfold size in *. contradict H.
+  rewrite N.eqb_compare. rewrite N.compare_refl. easy.
+Qed.
+*)
+
+Lemma bv_or_comm: forall a b, (size a) = _size -> (size b) = _size -> bv_or a b = bv_or b a.
+Admitted.
+(*
+Proof. intros a b H0 H1. unfold bv_or.
+       rewrite H0, H1. rewrite N.eqb_compare. rewrite N.compare_refl.
+       rewrite map2_or_comm. reflexivity.
+Qed.
+*)
+
+Lemma bv_or_assoc: forall a b c, (size a) = _size -> (size b) = _size -> (size c) = _size ->  
+                                  (bv_or a (bv_or b c)) = (bv_or (bv_or a b) c).
+Admitted.
+(*
+Proof. intros a b c H0 H1 H2. 
+       unfold bv_or. rewrite H1, H2.  
+       rewrite N.eqb_compare. rewrite N.eqb_compare. rewrite N.compare_refl.
+       unfold size, bits in *.
+       rewrite N.compare_refl.
+       rewrite N.eqb_compare.
+       rewrite N.compare_refl.
+       rewrite map2_or_assoc. reflexivity.
+Qed.
+*)
+
+(*
+
+Lemma bv_or_nth_bitOf: forall a b n (i: nat), 
+                          (size a) = n -> (size b) = n ->
+                          (i <= (nat_of_N (size a)))%nat ->
+                          nth i (bits (bv_or a b)) false = (nth i (bits a) false) || (nth i (bits b) false).
+Proof. intros a b n i H0 H1 H2. 
+       unfold bv_or. rewrite H0, H1. rewrite N.eqb_compare. rewrite N.compare_refl.
+       apply map2_or_nth_bitOf; unfold size in *; unfold bits.
+       now rewrite <- Nat2N.inj_iff, H1. rewrite Nat2N.id in H2; exact H2.
+Qed.
+
+
+
+Lemma bv_or_0_neutral: forall a, (bv_or a (mk_list_false (length (bits a)))) = a.
+Proof. intro a. unfold bv_or.
+       rewrite N.eqb_compare. unfold size, bits. 
+       rewrite N.compare_refl.
+       rewrite map2_or_0_neutral. reflexivity.
+Qed.
+
+Lemma bv_or_1_true: forall a, (bv_or a (mk_list_true (length (bits a)))) = (mk_list_true (length (bits a))).
+Proof. intro a. unfold bv_or.
+       rewrite N.eqb_compare.  unfold size, bits.
+       rewrite N.compare_refl.
+       rewrite map2_or_1_true. reflexivity.
+Qed.
+
+*)
+
+(* lists bitwise XOR properties *)
+
+Definition size_bv_xor (a b: bitvector) := _size.
+
+Lemma map2_xor_comm: forall (a b: list bool), (map2 xorb a b) = (map2 xorb b a).
+Proof. intros a. induction a as [ | a' xs IHxs].
+       intros [ | b' ys].
+       - simpl. auto.
+       - simpl. auto.
+       - intros [ | b' ys].
+         + simpl. auto.
+         + intros. simpl. 
+           cut (xorb a' b' = xorb b' a'). intro H. rewrite <- H. apply f_equal.
+           apply IHxs. apply xorb_comm.
+Qed.
+
+
+Lemma map2_xor_assoc: forall (a b c: list bool), (map2 xorb a (map2 xorb b c)) = (map2 xorb (map2 xorb a b) c).
+Proof. intro a. induction a as [ | a' xs IHxs].
+       simpl. auto.
+       intros [ | b' ys].
+        -  simpl. auto.
+        - intros [ | c' zs].
+          + simpl. auto.
+          + simpl. cut (xorb a' (xorb b' c') = (xorb (xorb a'  b')  c')). intro H. rewrite <- H. apply f_equal.
+            apply IHxs. rewrite xorb_assoc_reverse. reflexivity.
+Qed.
+
+Lemma map2_xor_length: forall (a b: list bool), length a = length b -> length a = length (map2 xorb a b).
+Proof. induction a as [ | a' xs IHxs].
+       simpl. auto.
+       intros [ | b ys].
+       - simpl. intros. exact H.
+       - intros. simpl in *. apply f_equal. apply IHxs.
+         inversion H; auto.
+Qed.
+
+Lemma map2_xor_empty_empty1:  forall (a: list bool), (map2 xorb a []) = [].
+Proof. intros a. induction a as [ | a' xs IHxs]; simpl; auto. Qed.
+
+Lemma map2_xor_empty_empty2:  forall (a: list bool), (map2 xorb [] a) = [].
+Proof. intros a. rewrite map2_xor_comm. apply map2_xor_empty_empty1. Qed.
+
+Lemma map2_xor_nth_bitOf: forall (a b: list bool) (i: nat), 
+                          (length a) = (length b) ->
+                          (i <= (length a))%nat ->
+                          nth i (map2 xorb a b) false = xorb (nth i a false) (nth i b false).
+Proof. intro a.
+       induction a as [ | a xs IHxs].
+         - intros [ | b ys].
+           + intros i H0 H1. do 2 rewrite map2_nth_empty_false. reflexivity.
+           + intros i H0 H1. rewrite map2_xor_empty_empty2.
+             rewrite map2_nth_empty_false. contradict H1. simpl. unfold not. intros. easy.
+         - intros [ | b ys].
+           + intros i H0 H1. rewrite map2_xor_empty_empty1.
+             rewrite map2_nth_empty_false. rewrite xorb_false_r. rewrite H0 in H1.
+             contradict H1. simpl. unfold not. intros. easy.
+           + intros i H0 H1. simpl.
+             revert i H1. intros [ | i IHi].
+             * simpl. auto.
+             * apply IHxs.
+                 inversion H0; reflexivity.
+                 inversion IHi; lia.
+Qed.
+
+(*bitvector XOR properties*)
+
+Lemma bv_xor_size a b: size (bv_xor a b) = _size.
+Admitted.
+(*
+Proof.
+  unfold bv_xor.
+  case_eq (size a =? size b); intros.
+  - rewrite N.eqb_eq in H. now unfold size in *.
+  - unfold size in *.
+    contradict H. rewrite N.eqb_compare, N.compare_refl. easy.
+Qed.
+*)
+
+Lemma bv_xor_comm: forall a b, (size a) = _size -> (size b) = _size -> bv_xor a b = bv_xor b a.
+Admitted.
+(*
+Proof. intros a b H0 H1. unfold bv_xor.
+       rewrite H0, H1. rewrite N.eqb_compare. rewrite N.compare_refl.
+       rewrite map2_xor_comm. reflexivity.
+Qed.
+*)
+
+Lemma bv_xor_assoc: forall a b c, (size a) = _size -> (size b) = _size -> (size c) = _size ->  
+                                  (bv_xor a (bv_xor b c)) = (bv_xor (bv_xor a b) c).
+Admitted.
+(*
+Proof. intros a b c H0 H1 H2. 
+       unfold bv_xor. rewrite H1, H2.  
+       rewrite N.eqb_compare. rewrite N.eqb_compare. rewrite N.compare_refl.
+       unfold size, bits in *.
+       rewrite N.compare_refl.
+       rewrite N.eqb_compare.
+       rewrite N.compare_refl.
+       rewrite map2_xor_assoc; reflexivity.
+Qed.
+*)
+
+(*
+
+Lemma bv_xor_empty_empty1: forall a, (bv_xor a bv_empty) = bv_empty.
+Proof. intros a. unfold bv_empty. 
+       unfold bv_xor, bits, size. simpl.
+       case_eq (N.compare (N.of_nat (length a)) 0); intro H; simpl.
+         - apply (N.compare_eq (N.of_nat (length a)) 0) in H.
+         
+           rewrite H. simpl. rewrite map2_xor_empty_empty1; reflexivity.
+         - rewrite N.eqb_compare. rewrite H; reflexivity.
+         - rewrite N.eqb_compare. rewrite H; reflexivity.
+Qed.
+
+Lemma bv_xor_nth_bitOf: forall a b n (i: nat), 
+                          (size a) = n -> (size b) = n ->
+                          (i <= (nat_of_N (size a)))%nat ->
+                          nth i (bits (bv_xor a b)) false = xorb (nth i (bits a) false) (nth i (bits b) false).
+Proof. intros a b n i H0 H1 H2. 
+       unfold bv_xor. rewrite H0, H1. rewrite N.eqb_compare. rewrite N.compare_refl.
+       apply map2_xor_nth_bitOf; unfold size in *; unfold bits.
+       now rewrite <- Nat2N.inj_iff, H1. rewrite Nat2N.id in H2; exact H2.
+Qed.
+
+
+Lemma bv_xor_0_neutral: forall a, (bv_xor a (mk_list_false (length (bits a)))) = a.
+Proof. intro a. unfold bv_xor.
+       rewrite N.eqb_compare. unfold size, bits.
+       rewrite N.compare_refl.
+       rewrite map2_xor_0_neutral. reflexivity.
+Qed.
+
+Lemma bv_xor_1_true: forall a, (bv_xor a (mk_list_true (length (bits a)))) = map negb a.
+Proof. intro a. unfold bv_xor.
+       rewrite N.eqb_compare.  unfold size, bits.
+       rewrite N.compare_refl.
+       rewrite map2_xor_1_true. reflexivity.
+Qed.
+*)
+
+(*bitwise NOT properties*)
+
+Lemma not_list_length: forall a, length a = length (map negb a).
+Proof. intro a.
+       induction a as [ | a xs IHxs].
+       - auto. 
+       - simpl. apply f_equal. exact IHxs.
+Qed.
+
+Lemma not_list_involutative: forall a, map negb (map negb a) = a.
+Proof. intro a.
+       induction a as [ | a xs IHxs]; auto.
+       simpl. rewrite negb_involutive. apply f_equal. exact IHxs.
+Qed.
+
+Lemma not_list_and_or: forall a b, map negb (map2 andb a b) = map2 orb (map negb a) (map negb b).
+Proof. intro a.
+       induction a as [ | a xs IHxs].
+       - auto.
+       - intros [ | b ys].
+         + auto.
+         + simpl. rewrite negb_andb. apply f_equal. apply IHxs.
+Qed.
+
+Lemma not_list_or_and: forall a b, map negb (map2 orb a b) = map2 andb (map negb a) (map negb b).
+Proof. intro a.
+       induction a as [ | a xs IHxs].
+       - auto.
+       - intros [ | b ys].
+         + auto.
+         + simpl. rewrite negb_orb. apply f_equal. apply IHxs.
+Qed.
+
+(*
+(*bitvector NOT properties*)
+
+Lemma bv_not_size: forall a, (size a) = _size -> size (bv_not a) = _size.
+Proof. intros a H. unfold bv_not. now unfold size, bits in *. Qed.
+
+Lemma bv_not_involutative: forall a, bv_not (bv_not a) = a.
+Proof. intro a. unfold bv_not.
+       unfold size, bits. rewrite not_list_involutative. reflexivity.
+Qed.
+
+Lemma bv_not_false_true: forall n, bv_not (mk_list_false n) = (mk_list_true n).
+Proof. intros n. unfold bv_not.
+       unfold size, bits. rewrite not_list_false_true. reflexivity.
+Qed.
+
+Lemma bv_not_true_false: forall n, bv_not (mk_list_true n) = (mk_list_false n).
+Proof. intros n. unfold bv_not.
+       unfold size, bits. rewrite not_list_true_false. reflexivity.
+Qed.
+*)
+
+(*
+Lemma bv_not_and_or: forall n a b, (size a) = n -> (size b) = n -> bv_not (bv_and a b) = bv_or (bv_not a) (bv_not b).
+Proof. intros n a b H0 H1. unfold bv_and in *.
+       rewrite H0, H1. rewrite N.eqb_compare. rewrite N.compare_refl.
+       unfold bv_or, size, bits in *.
+       do 2 rewrite <- not_list_length. rewrite H0, H1.
+       rewrite N.eqb_compare. rewrite N.compare_refl. 
+       unfold bv_not, size, bits in *. 
+       rewrite not_list_and_or. reflexivity.
+Qed.
+
+Lemma bv_not_or_and: forall n a b, (size a) = n -> (size b) = n -> bv_not (bv_or a b) = bv_and (bv_not a) (bv_not b).
+Proof. intros n a b H0 H1. unfold bv_and, size, bits in *. 
+       do 2 rewrite <- not_list_length.
+       rewrite H0, H1. rewrite N.eqb_compare. rewrite N.compare_refl.
+       unfold bv_or, size, bits in *.
+       rewrite H0, H1. rewrite N.eqb_compare. rewrite N.compare_refl. 
+       unfold bv_not, size, bits in *.
+       rewrite not_list_or_and. reflexivity.
+Qed.
+*)
+
+(* list bitwise ADD properties*)
+
+Definition size_bv_add (a b: bitvector) := _size.
+
+Lemma add_carry_ff: forall a, add_carry a false false = (a, false).
+Proof. intros a.
+       case a; simpl; auto.
+Qed.
+
+Lemma add_carry_neg_f: forall a, add_carry a (negb a) false = (true, false).
+Proof. intros a.
+       case a; simpl; auto.
+Qed.
+
+Lemma add_carry_neg_f_r: forall a, add_carry (negb a) a false = (true, false).
+Proof. intros a.
+       case a; simpl; auto.
+Qed.
+
+Lemma add_carry_neg_t: forall a, add_carry a (negb a) true = (false, true).
+Proof. intros a.
+       case a; simpl; auto.
+Qed.
+
+Lemma add_carry_tt: forall a, add_carry a true true = (a, true).
+Proof. intro a. case a; auto. Qed.
+
+Lemma add_list_empty_l: forall (a: list bool), (add_list [] a) = [].
+Proof. intro a. induction a as [ | a xs IHxs].
+         - unfold add_list. simpl. reflexivity.
+         - apply IHxs.
+Qed.
+
+Lemma add_list_empty_r: forall (a: list bool), (add_list a []) = [].
+Proof. intro a. induction a as [ | a xs IHxs]; unfold add_list; simpl; reflexivity. Qed.
+
+Lemma add_list_ingr_l: forall (a: list bool) (c: bool), (add_list_ingr [] a c) = [].
+Proof. intro a. induction a as [ | a xs IHxs]; unfold add_list; simpl; reflexivity. Qed.
+
+Lemma add_list_ingr_r: forall (a: list bool) (c: bool), (add_list_ingr a [] c) = [].
+Proof. intro a. induction a as [ | a xs IHxs]; unfold add_list; simpl; reflexivity. Qed.
+
+Lemma add_list_carry_comm: forall (a b:  list bool) (c: bool), add_list_ingr a b c = add_list_ingr b a c.
+Proof. intros a. induction a as [ | a' xs IHxs]; intros b c.
+       - simpl. rewrite add_list_ingr_r. reflexivity.
+       - case b as [ | b' ys].
+         + simpl. auto.
+         + simpl in *. cut (add_carry a' b' c = add_carry b' a' c).
+           * intro H. rewrite H. destruct (add_carry b' a' c) as (r, c0).
+             rewrite IHxs. reflexivity.
+           * case a', b', c;  auto.
+Qed.
+
+Lemma add_list_comm: forall (a b: list bool), (add_list a b) = (add_list b a).
+Proof. intros a b. unfold add_list. apply (add_list_carry_comm a b false). Qed.
+
+Lemma add_list_carry_assoc: forall (a b c:  list bool) (d1 d2 d3 d4: bool),
+                            add_carry d1 d2 false = add_carry d3 d4 false ->
+                            (add_list_ingr (add_list_ingr a b d1) c d2) = (add_list_ingr a (add_list_ingr b c d3) d4).
+Proof. intros a. induction a as [ | a' xs IHxs]; intros b c d1 d2 d3 d4.
+       - simpl. reflexivity.
+       - case b as [ | b' ys].
+         + simpl. auto.
+         + case c as [ | c' zs].
+           * simpl. rewrite add_list_ingr_r. auto.
+           * simpl.
+             case_eq (add_carry a' b' d1); intros r0 c0 Heq0. simpl.
+             case_eq (add_carry r0 c' d2); intros r1 c1 Heq1.
+             case_eq (add_carry b' c' d3); intros r3 c3 Heq3.
+             case_eq (add_carry a' r3 d4); intros r2 c2 Heq2.
+             intro H. rewrite (IHxs _ _ c0 c1 c3 c2);
+               revert Heq0 Heq1 Heq3 Heq2;
+               case a', b', c', d1, d2, d3, d4; simpl; do 4 (intros H'; inversion_clear H'); 
+               (*; intros H'; inversion_clear H'; intros H'; inversion_clear H'; intros H'; inversion_clear H'; *)
+                 try reflexivity; simpl in H; discriminate.
+Qed.
+
+Lemma add_list_carry_length_eq: forall (a b: list bool) c, length a = length b -> length a = length (add_list_ingr a b c).
+Proof. induction a as [ | a' xs IHxs].
+       simpl. auto.
+       intros [ | b ys].
+       - simpl. intros. exact H.
+       - intros. simpl in *.
+         case_eq (add_carry a' b c); intros r c0 Heq. simpl. apply f_equal.
+         specialize (@IHxs ys). apply IHxs. inversion H; reflexivity.
+Qed.
+
+Lemma add_list_carry_length_ge: forall (a b: list bool) c, (length a >= length b)%nat -> length b = length (add_list_ingr a b c).
+Proof. induction a as [ | a' xs IHxs].
+       simpl. intros b H0 H1. lia.
+       intros [ | b ys].
+       - simpl. intros. auto.
+       - intros. simpl in *.
+         case_eq (add_carry a' b c); intros r c0 Heq. simpl. apply f_equal.
+         specialize (@IHxs ys). apply IHxs. lia.
+Qed.
+
+Lemma add_list_carry_length_le: forall (a b: list bool) c, (length b >= length a)%nat -> length a = length (add_list_ingr a b c).
+Proof. induction a as [ | a' xs IHxs].
+       simpl. intros b H0 H1. reflexivity.
+       intros [ | b ys].
+       - simpl. intros. contradict H. lia.
+       - intros. simpl in *.
+         case_eq (add_carry a' b c); intros r c0 Heq. simpl. apply f_equal.
+         specialize (@IHxs ys). apply IHxs. lia.
+Qed.
+
+Lemma length_add_list_eq: forall (a b: list bool), length a = length b -> length a = length (add_list a b).
+Proof. intros a b H. unfold add_list. apply (@add_list_carry_length_eq a b false). exact H. Qed.
+
+Lemma length_add_list_ge: forall (a b: list bool), (length a >= length b)%nat -> length b = length (add_list a b).
+Proof. intros a b H. unfold add_list. apply (@add_list_carry_length_ge a b false). exact H. Qed.
+
+Lemma length_add_list_le: forall (a b: list bool), (length b >= length a)%nat -> length a = length (add_list a b).
+Proof. intros a b H. unfold add_list. apply (@add_list_carry_length_le a b false). exact H. Qed.
+
+Lemma add_list_assoc: forall (a b c: list bool), (add_list (add_list a b) c) = (add_list a (add_list b c)).
+Proof. intros a b c. unfold add_list.
+       apply (@add_list_carry_assoc a b c false false false false).
+       simpl; reflexivity.
+Qed.
+
+Lemma add_list_carry_empty_neutral_n_l: forall (a: list bool) n, (n >= (length a))%nat -> (add_list_ingr (mk_list_false n) a false) = a.
+Proof. intro a. induction a as [ | a' xs IHxs].
+       - intro n. rewrite add_list_ingr_r. reflexivity.
+       - intros [ | n]. 
+         + simpl. intro H. contradict H. easy.
+         + simpl. intro H.
+           case a'; apply f_equal; apply IHxs; lia.
+Qed.
+
+Lemma add_list_carry_empty_neutral_n_r: forall (a: list bool) n, (n >= (length a))%nat -> (add_list_ingr a (mk_list_false n) false) = a.
+Proof. intro a. induction a as [ | a' xs IHxs].
+       - intro n. rewrite add_list_ingr_l. reflexivity.
+       - intros [ | n]. 
+         + simpl. intro H. contradict H. easy.
+         + simpl. intro H.
+           case a'; apply f_equal; apply IHxs; lia.
+Qed.
+
+Lemma add_list_carry_empty_neutral_l: forall (a: list bool), (add_list_ingr (mk_list_false (length a)) a false) = a.
+Proof. intro a.
+       rewrite add_list_carry_empty_neutral_n_l; auto.
+Qed.
+
+Lemma add_list_carry_empty_neutral_r: forall (a: list bool), (add_list_ingr a (mk_list_false (length a)) false) = a.
+Proof. intro a.
+       rewrite add_list_carry_empty_neutral_n_r; auto.
+Qed.
+
+Lemma add_list_empty_neutral_n_l: forall (a: list bool) n, (n >= (length a))%nat -> (add_list (mk_list_false n) a) = a.
+Proof. intros a. unfold add_list.
+       apply (@add_list_carry_empty_neutral_n_l a).
+Qed.
+
+Lemma add_list_empty_neutral_n_r: forall (a: list bool) n, (n >= (length a))%nat -> (add_list a (mk_list_false n)) = a.
+Proof. intros a. unfold add_list.
+       apply (@add_list_carry_empty_neutral_n_r a).
+Qed.
+
+Lemma add_list_empty_neutral_r: forall (a: list bool), (add_list a (mk_list_false (length a))) = a.
+Proof. intros a. unfold add_list.
+       apply (@add_list_carry_empty_neutral_r a).
+Qed.
+
+Lemma add_list_empty_neutral_l: forall (a: list bool), (add_list (mk_list_false (length a)) a) = a.
+Proof. intros a. unfold add_list.
+       apply (@add_list_carry_empty_neutral_l a).
+Qed.
+
+
+Lemma add_list_carry_twice: forall a c, add_list_ingr a a c = removelast (c :: a).
+Proof. intro a. 
+       induction a as [ | a xs IHxs].
+       - intros c. simpl. reflexivity.
+       - intros [ | ].
+         + simpl. case a.
+           * simpl. rewrite IHxs.
+             case_eq xs. intro Heq0. simpl. reflexivity.
+             reflexivity.
+           * simpl. rewrite IHxs.
+             case_eq xs. intro Heq0. simpl. reflexivity.
+             reflexivity.
+         + simpl. case a.
+           * simpl. rewrite IHxs.
+             case_eq xs. intro Heq0. simpl. reflexivity.
+             reflexivity.
+           * simpl. rewrite IHxs.
+             case_eq xs. intro Heq0. simpl. reflexivity.
+             reflexivity.
+Qed.
+
+Lemma add_list_twice: forall a, add_list a a = removelast (false :: a).
+Proof. intro a. 
+       unfold add_list. rewrite add_list_carry_twice. reflexivity.
+Qed.
+
+(*bitvector ADD properties*)
+
+Lemma bv_add_size a b: size (bv_add a b) = _size.
+Admitted.
+(*
+Proof.
+  unfold bv_add.
+  case_eq (size a =? size b); intros.
+  - rewrite N.eqb_eq in H. now unfold size in *.
+  - unfold size in *. contradict H.
+    rewrite N.eqb_compare, N.compare_refl. easy.
+Qed.
+*)
+
+Lemma bv_add_comm: forall a b, (size a) = _size -> (size b) = _size -> bv_add a b = bv_add b a.
+Admitted.
+(*
+Proof. intros a b H0 H1.
+       unfold bv_add, size, bits in *.
+       rewrite N.eqb_compare. rewrite N.compare_refl.
+       rewrite add_list_comm. reflexivity.
+Qed.
+*)
+
+Lemma bv_add_assoc: forall a b c, (size a) = _size -> (size b) = _size -> (size c) = _size ->  
+                                  (bv_add a (bv_add b c)) = (bv_add (bv_add a b) c).
+Admitted.
+(*
+Proof. intros a b c H0 H1 H2.
+       unfold bv_add, size, bits in *.
+       rewrite N.eqb_compare. rewrite N.compare_refl.
+       rewrite add_list_assoc. reflexivity.
+Qed.
+*)
+
+(*
+Lemma bv_add_empty_neutral_l: forall a, (bv_add (mk_list_false (length (bits a))) a) = a.
+Proof. intro a. unfold bv_add, size, bits. 
+       rewrite N.eqb_compare. rewrite N.compare_refl.
+       rewrite add_list_empty_neutral_l. reflexivity.
+Qed.
+
+Lemma bv_add_empty_neutral_r: forall a, (bv_add a (mk_list_false (length (bits a)))) = a.
+Proof. intro a. unfold bv_add, size, bits.
+       rewrite N.eqb_compare. rewrite N.compare_refl.
+       rewrite add_list_empty_neutral_r. reflexivity.
+Qed.
+
+Lemma bv_add_twice: forall a, bv_add a a = removelast (false :: a).
+Proof. intro a. unfold bv_add, size, bits.
+       rewrite N.eqb_compare. rewrite N.compare_refl.
+       rewrite add_list_twice. reflexivity.
+Qed.
+*)
+
+(* bitwise SUBST properties *)
+
+
+
+Definition size_bv_subst (a b: bitvector) := _size.
+
+Lemma subst_list_empty_empty_l: forall a, (subst_list [] a) = [].
+Proof. intro a. unfold subst_list; auto. Qed.
+
+Lemma subst_list_empty_empty_r: forall a, (subst_list a []) = [].
+Proof. intro a.
+       induction a as [ | a xs IHxs].
+       - auto.
+       - unfold subst_list; auto. 
+Qed.
+
+Lemma subst_list'_empty_empty_r: forall a, (subst_list' a []) = [].
+Proof. intro a.
+       induction a as [ | a xs IHxs].
+       - auto.
+       - unfold subst_list' in *. unfold twos_complement. simpl. reflexivity.
+Qed.
+
+Lemma subst_list_borrow_length: forall (a b: list bool) c, length a = length b -> length a = length (subst_list_borrow a b c). 
+Proof. induction a as [ | a' xs IHxs]. 
+       simpl. auto. 
+       intros [ | b ys].
+       - simpl. intros. exact H. 
+       - intros. simpl in *. 
+         case_eq (subst_borrow a' b c); intros r c0 Heq. simpl. apply f_equal. 
+         specialize (@IHxs ys). apply IHxs. inversion H; reflexivity. 
+Qed.
+
+Lemma length_twos_complement: forall (a: list bool), length a = length (twos_complement a).
+Proof. intro a.
+      induction a as [ | a' xs IHxs].
+      - auto.
+      - unfold twos_complement. specialize (@add_list_carry_length_eq (map negb (a' :: xs)) (mk_list_false (length (a' :: xs))) true).        
+        intro H. rewrite <- H. simpl. apply f_equal. rewrite <- not_list_length. reflexivity.
+        rewrite length_mk_list_false. rewrite <- not_list_length. reflexivity.
+Qed.
+
+Lemma subst_list_length: forall (a b: list bool), length a = length b -> length a = length (subst_list a b). 
+Proof. intros a b H. unfold subst_list. apply (@subst_list_borrow_length a b false). exact H. Qed.
+
+Lemma subst_list'_length: forall (a b: list bool), length a = length b -> length a = length (subst_list' a b).
+Proof. intros a b H. unfold subst_list'.
+       rewrite <- (@length_add_list_eq a (twos_complement b)).
+       - reflexivity.
+       - rewrite <- (@length_twos_complement b). exact H.
+Qed.
+
+Lemma subst_list_borrow_empty_neutral: forall (a: list bool), (subst_list_borrow a (mk_list_false (length a)) false) = a.
+Proof. intro a. induction a as [ | a' xs IHxs].
+       - simpl. reflexivity.
+       - simpl.
+         cut(subst_borrow a' false false = (a', false)).
+         + intro H. rewrite H. rewrite IHxs. reflexivity.
+         + unfold subst_borrow. case a'; auto.
+Qed.
+
+Lemma subst_list_empty_neutral: forall (a: list bool), (subst_list a (mk_list_false (length a))) = a.
+Proof. intros a. unfold subst_list.
+       apply (@subst_list_borrow_empty_neutral a).
+Qed.
+
+Lemma twos_complement_cons_false: forall a, false :: twos_complement a = twos_complement (false :: a).
+Proof. intro a.
+       induction a as [ | a xs IHxs]; unfold twos_complement; simpl; reflexivity.
+Qed.
+
+Lemma twos_complement_false_false: forall n, twos_complement (mk_list_false n) = mk_list_false n.
+Proof. intro n.
+       induction n as [ | n IHn].
+       - auto.
+       - simpl. rewrite <- twos_complement_cons_false.
+         apply f_equal. exact IHn.
+Qed.
+
+Lemma subst_list'_empty_neutral: forall (a: list bool), (subst_list' a (mk_list_false (length a))) = a.
+Proof. intros a. unfold subst_list'.
+       rewrite (@twos_complement_false_false (length a)).
+       rewrite add_list_empty_neutral_r. reflexivity.
+Qed.
+
+(* bitvector SUBST properties *)
+
+Lemma bv_subst_size a b: size (bv_subst a b) = _size.
+Admitted.
+(*
+Proof.
+  unfold bv_subst.
+  case_eq (size a =? size b); intros.
+  - rewrite N.eqb_eq in H. now unfold size in *.
+  - unfold size in *. contradict H.
+    rewrite N.eqb_compare, N.compare_refl. easy.
+Qed.
+
+Lemma bv_subst_empty_neutral_r: forall a, (bv_subst a  (mk_list_false (length (bits a)))) = a.
+Proof. intro a. unfold bv_subst, size, bits.
+       rewrite N.eqb_compare.
+       rewrite N.compare_refl.
+       rewrite subst_list_empty_neutral. reflexivity.
+Qed.
+
+Lemma bv_subst'_size: forall a b, (size a) = _size -> (size b) = _size -> size (bv_subst' a b) = _size.
+Proof. intros a b H0 H1. now unfold bv_subst', size, bits in *. Qed.
+
+Lemma bv_subst'_empty_neutral_r: forall a, (bv_subst' a (mk_list_false (length (bits a)))) = a.
+Proof. intro a. unfold bv_subst', size, bits.
+       rewrite N.eqb_compare.
+       rewrite N.compare_refl.
+       rewrite subst_list'_empty_neutral. reflexivity.
+Qed.
+*)
+
+
+(*
+(* bitwise ADD-NEG properties *)
+
+Lemma add_neg_list_carry_false: forall a b c, add_list_ingr a (add_list_ingr b c true) false = add_list_ingr a (add_list_ingr b c false) true.
+Proof. intro a.
+       induction a as [ | a xs IHxs].
+       - simpl. auto.
+       - case b as [ | b ys].
+         + simpl. auto.
+         + case c as [ | c zs].
+           * simpl. auto.
+           * simpl.
+             case_eq (add_carry b c false); intros r0 c0 Heq0.
+             case_eq (add_carry b c true); intros r1 c1 Heq1.
+             case_eq (add_carry a r1 false); intros r2 c2 Heq2.
+             case_eq (add_carry a r0 true); intros r3 c3 Heq3.
+             case a, b, c; inversion Heq0; inversion Heq1; 
+             inversion Heq2; inversion Heq3; rewrite <- H2 in H4; 
+             rewrite <- H0 in H5; inversion H4; inversion H5; apply f_equal;
+             try reflexivity; rewrite IHxs; reflexivity.
+Qed.
+
+
+Lemma add_neg_list_carry_neg_f: forall a, (add_list_ingr a (map negb a) false) = mk_list_true (length a).
+Proof. intro a.
+       induction a as [ | a xs IHxs].
+       - simpl. reflexivity.
+       - simpl. 
+         case_eq (add_carry a (negb a) false); intros r0 c0 Heq0.
+         rewrite add_carry_neg_f in Heq0.
+         inversion Heq0. rewrite IHxs. reflexivity.
+Qed.
+
+Lemma add_neg_list_carry_neg_f_r: forall a, (add_list_ingr (map negb a) a false) = mk_list_true (length a).
+Proof. intro a.
+       induction a as [ | a xs IHxs].
+       - simpl. reflexivity.
+       - simpl. 
+         case_eq (add_carry (negb a) a false); intros r0 c0 Heq0.
+         rewrite add_carry_neg_f_r in Heq0.
+         inversion Heq0. rewrite IHxs. reflexivity.
+Qed.
+
+Lemma add_neg_list_carry_neg_t: forall a, (add_list_ingr a (map negb a) true) = mk_list_false (length a).
+Proof. intro a.
+       induction a as [ | a xs IHxs].
+       - simpl. reflexivity.
+       - simpl. 
+         case_eq (add_carry a (negb a) true); intros r0 c0 Heq0.
+         rewrite add_carry_neg_t in Heq0.
+         inversion Heq0. rewrite IHxs. reflexivity.
+Qed.
+
+Lemma add_neg_list_carry: forall a, add_list_ingr a (twos_complement a) false = mk_list_false (length a).
+Proof. intro a.
+       induction a as [ | a xs IHxs].
+       - simpl. reflexivity.
+       - unfold twos_complement. rewrite add_neg_list_carry_false. rewrite not_list_length at 1.
+         rewrite add_list_carry_empty_neutral_r.
+         rewrite add_neg_list_carry_neg_t. reflexivity.
+Qed.
+
+Lemma add_neg_list_absorb: forall a, add_list a (twos_complement a) = mk_list_false (length a).
+Proof. intro a. unfold add_list. rewrite add_neg_list_carry. reflexivity. Qed.
+
+*)
+
+(* bitwise MULT properties *)
+
+Definition size_bv_mult (a b: bitvector) := _size.
+
+
+Lemma mult_list_empty_l: forall (a: list bool), (mult_list [] a) = [].
+Proof. intro a. induction a as [ | a xs IHxs].
+         - unfold mult_list. simpl. reflexivity.
+         - apply IHxs.
+Qed.
+
+Lemma mult_list_carry_0: forall a b, mult_list_carry a b 0 = [].
+Proof. intro a. induction a as [ | a' xs IHxs].
+       - intro b. simpl. reflexivity.
+       - intros [ | b' ys].
+         + simpl. case_eq a'.
+           * simpl. intro H. rewrite add_list_empty_l; reflexivity.
+           * simpl. intro H. apply IHxs.
+         + simpl. case_eq a'.
+           * simpl. intro H. rewrite IHxs. rewrite add_list_empty_r; reflexivity.
+           * simpl. intro H. apply IHxs.
+Qed.
+
+Lemma mult_list_true: forall a n, ((length a) = n)%nat -> mult_list_carry [true] a n = a.
+Proof. intro a.
+       induction a as [ | a xs IHxs].
+       - intros n H. simpl in H. rewrite <- H.
+         rewrite mult_list_carry_0. reflexivity.
+       - intros [ | n] H.
+         + contradict H. easy.
+         + rewrite <- (IHxs n) at 2; try auto. simpl.
+           case a. unfold add_list. simpl. reflexivity.
+           unfold add_list. simpl. reflexivity.
+Qed.
+
+Lemma mult_list_false_l: forall a n, mult_list_carry [false] a n = mk_list_false n.
+Proof. intro a.
+       induction a as [ | a xs IHxs]; simpl; reflexivity.
+Qed.
+
+Lemma mult_list_carry_empty_l: forall (a: list bool) (c: nat), mult_list_carry [] a c = mk_list_false c.
+Proof. intro a. induction a as [ | a' xs IHxs]; auto. Qed.
+
+Lemma strictly_positive_0_unique: forall n: nat, (0 >= n)%nat <-> (n = 0)%nat.
+Proof. intro n. induction n as [ | n IHn].
+       split; try auto.
+       split; intro H; contradict H; easy.
+Qed.
+
+Lemma mult_list_carry_length: forall (a b: list bool) n, ((length b) >= n)%nat -> n = length (mult_list_carry a b n).
+Proof. intro a.
+       induction a as [ | a xs IHxs].
+       - intros b n H. rewrite mult_list_carry_empty_l, length_mk_list_false; reflexivity.
+       - intros [ | b ys] n H. simpl in H. rewrite strictly_positive_0_unique in H.
+         rewrite H. rewrite mult_list_carry_0. easy.
+         simpl. case a.
+         + specialize (@length_add_list_ge (b :: ys) (mult_list_carry xs (false :: b :: ys) n)).
+           intro H1. rewrite <- H1. 
+           rewrite <- (IHxs (false :: b :: ys)). reflexivity. simpl in *. lia.
+           specialize (@IHxs (false :: b :: ys)). rewrite <- IHxs. easy. simpl. simpl in H. lia.
+         + specialize (@IHxs (false :: b :: ys)). apply IHxs. inversion H. simpl. lia. simpl in *. lia.
+Qed.
+
+(* Lemma mult_list_length: forall (a b: list bool), ((length b) >= (length a))%nat -> (length a) = length (mult_list a b). *)
+(* Proof. intros a b H. unfold mult_list. *)
+(*        rewrite <- (@mult_list_carry_length a b (length a)); auto. *)
+(* Qed. *)
+
+(* Lemma mult_list_length_eq: forall (a b: list bool), ((length a) = (length b))%nat -> (length a) = length (mult_list a b). *)
+(* Proof. intros a b H. unfold mult_list. *)
+(*        rewrite <- (@mult_list_carry_length a b (length a)); lia. *)
+(* Qed. *)
+
+(* Lemma mult_list_cons_false1: forall (a b: list bool) n, ((length a) >= n)%nat -> ((length b) >= n)%nat -> *)
+(*                        mult_list_carry (false :: a) b n = mult_list_carry a (false :: b) n. *)
+(* Proof. intro a. *)
+(*        induction a as [ | a xs IHxs]. *)
+(*        - intros b n H0 H1. rewrite strictly_positive_0_unique in H0. rewrite H0. *)
+(*          do 2 rewrite mult_list_carry_0. reflexivity. *)
+(*        - intros [ | b ys] n H0 H1. *)
+(*          + rewrite strictly_positive_0_unique in H1. rewrite H1. *)
+(*            do 2 rewrite mult_list_carry_0. reflexivity. *)
+(*          + simpl. reflexivity. *)
+(* Qed. *)
+
+(* Lemma mult_list_cons_false1': forall (a b: list bool) n, ((length (false :: b)) >= n)%nat -> *)
+(*                        mult_list_carry (false :: a) b n = mult_list_carry a (false :: b) n. *)
+(* Proof. intro a. *)
+(*        induction a as [ | a xs IHxs]. *)
+(*        - intros b n H0. rewrite mult_list_carry_empty_l. simpl. reflexivity. *)
+(*        - intros [ | b ys] n H0. *)
+(*          + simpl. case a; reflexivity. *)
+(*          + simpl. reflexivity. *)
+(* Qed. *)
+
+(* Lemma mult_list_cons_false1'': forall (a b: list bool) n, *)
+(*                        mult_list_carry (false :: a) b n = mult_list_carry a (false :: b) n. *)
+(* Proof. intro a. *)
+(*        induction a as [ | a xs IHxs]. *)
+(*        - intros b n. rewrite mult_list_carry_empty_l. simpl. reflexivity. *)
+(*        - intros [ | b ys] n. *)
+(*          + simpl. case a; reflexivity. *)
+(*          + simpl. reflexivity. *)
+(* Qed. *)
+
+(* Lemma mult_list_cons_false2: forall (a b: list bool) n, ((length a) >= n)%nat -> ((length b) >= n)%nat -> *)
+(*                        mult_list_carry a (false :: b) n = mult_list_carry (false :: a) b n. *)
+(* Proof. intro a. *)
+(*        induction a as [ | a xs IHxs]. *)
+(*        - intros b n H0 H1. rewrite strictly_positive_0_unique in H0. rewrite H0. *)
+(*          do 2 rewrite mult_list_carry_0. reflexivity. *)
+(*        - intros [ | b ys] n H0 H1. *)
+(*          + rewrite strictly_positive_0_unique in H1. rewrite H1. *)
+(*            do 2 rewrite mult_list_carry_0. reflexivity. *)
+(*          + simpl. reflexivity. *)
+(* Qed. *)
+
+(* Lemma mult_list_cons_false2': forall (a b: list bool) n, ((length (false :: b)) >= n)%nat -> *)
+(*                        mult_list_carry a (false :: b) n = mult_list_carry (false :: a) b n. *)
+(* Proof. intro a. *)
+(*        induction a as [ | a xs IHxs]. *)
+(*        - intros b n H0. rewrite mult_list_carry_empty_l. simpl. reflexivity. *)
+(*        - intros [ | b ys] n H0. *)
+(*          + simpl. case a; reflexivity. *)
+(*          + simpl. reflexivity. *)
+(* Qed. *)
+
+(* Lemma mult_list_cons_false2'': forall (a b: list bool) n, *)
+(*                        mult_list_carry a (false :: b) n = mult_list_carry (false :: a) b n. *)
+(* Proof. intro a. *)
+(*        induction a as [ | a xs IHxs]. *)
+(*        - intros b n. rewrite mult_list_carry_empty_l. simpl. reflexivity. *)
+(*        - intros [ | b ys] n. *)
+(*          + simpl. case a; reflexivity. *)
+(*          + simpl. reflexivity. *)
+(* Qed. *)
+
+Lemma add_list_carry_rl0: forall (a b: list bool), 
+add_list_ingr (add_list_ingr a a false) b false = add_list_ingr (removelast (false :: a)) b false.
+Proof. intros a b. now rewrite add_list_carry_twice. Qed.
+
+Lemma add_list_carry_rl1: forall (a b: list bool), 
+add_list_ingr (removelast (false :: a)) b true = add_list_ingr (removelast (true :: a)) b false.
+Proof. intros a b.
+       simpl. case a.
+       simpl. reflexivity.
+       intros b0 l.
+       simpl. reflexivity.
+Qed.
+
+Lemma add_list_carry_rl_t: forall  (a b: list bool), a <> [] ->
+add_list_ingr (removelast (true :: a)) b false =
+add_list_ingr a (add_list_ingr a b false) true.
+Proof. intro a.
+       induction a as [ | a xs IHxs].
+       - intros b H0. now contradict H0.
+       - intros [ | b ys] H0.
+         + reflexivity.
+         + case a, b; 
+           do 4 (rewrite <- (@add_list_carry_assoc _ _ _ false true); 
+                 [rewrite add_list_carry_twice; rewrite  add_list_carry_rl1; reflexivity| auto]).
+Qed.
+
+Lemma add_list_carry_tf_t: forall (a b: list bool),
+add_list (true :: a) (false :: b) = true :: add_list a b.
+Proof. now simpl. Qed.
+
+Lemma add_list_carry_ft_t: forall (a b: list bool),
+add_list (false :: a) (true :: b) = true :: add_list a b.
+Proof. now simpl. Qed.
+
+Lemma add_list_carry_tf_tf_comm: forall (a b: list bool),
+(add_list (true :: a) (false :: b)) = (add_list (true :: b) (false :: a)).
+Proof. intro a.
+       induction a as [ | a xs IHxs].
+       - intros [ | b ys].
+         + reflexivity.
+         + simpl. now do 2 rewrite add_list_carry_tf_t.
+       - intros [ | b ys].
+         + simpl. now do 2 rewrite add_list_carry_tf_t.
+         + do 2 rewrite add_list_carry_tf_t. apply f_equal.
+           case a, b; now rewrite add_list_comm.
+Qed.
+
+Lemma add_list_carry_ft_ft_comm: forall (a b: list bool),
+(add_list (false :: a) (true :: b)) = (add_list (false :: b) (true :: a)).
+Proof. intro a.
+       induction a as [ | a xs IHxs]; intros [ | b ys]; try (now unfold add_list).
+       unfold add_list. simpl. apply f_equal.
+       case a, b; simpl; now rewrite add_list_carry_comm.
+Qed.
+
+Lemma add_list_carry_ff_f: forall (a b: list bool),
+(add_list (false :: a) (false :: b)) = (false :: add_list a b).
+Proof. intro a.
+       induction a as [ | a xs IHxs]; intros [ | b ys]; now unfold add_list.
+Qed.
+
+(* Lemma mult_list_carry_f_f_1: forall (a b: list bool) n, *)
+(*                        mult_list_carry (false :: a) b (S n) = false :: mult_list_carry a b n. *)
+(* Proof. intro a. *)
+(*        induction a as [ | a xs IHxs]. *)
+(*        - intros b n. rewrite mult_list_carry_empty_l. simpl. reflexivity. *)
+(*        - intros [ | b ys] n. *)
+(*          + case a. *)
+(*           * rewrite mult_list_cons_false1''.  *)
+(*             simpl. rewrite mult_list_cons_false2''. *)
+(*             rewrite IHxs. *)
+(*             rewrite mult_list_cons_false2''. *)
+(*             now rewrite <- add_list_carry_ff_f. *)
+(*           * rewrite mult_list_cons_false1''.  *)
+(*             simpl. rewrite mult_list_cons_false2''. *)
+(*             rewrite IHxs. *)
+(*             now rewrite mult_list_cons_false2''. *)
+(*          + case a, b. *)
+(*            * simpl. rewrite mult_list_cons_false2''. rewrite IHxs. *)
+(*              now rewrite add_list_carry_ff_f. *)
+(*            * simpl. rewrite mult_list_cons_false2''. rewrite IHxs. *)
+(*              now rewrite add_list_carry_ff_f. *)
+(*            * simpl. rewrite mult_list_cons_false2''. *)
+(*              rewrite IHxs. reflexivity. *)
+(*            * simpl. rewrite mult_list_cons_false2''. *)
+(*              rewrite IHxs. reflexivity. *)
+(* Qed. *)
+
+(* Lemma mult_list_carry_f_f_2: forall (a b: list bool) n, *)
+(*                        mult_list_carry a (false :: b) (S n) = false :: mult_list_carry a b n. *)
+(* Proof. intro a. *)
+(*        induction a as [ | a xs IHxs]. *)
+(*        - intros b n. rewrite mult_list_carry_empty_l. simpl. reflexivity. *)
+(*        - intros [ | b ys] n. *)
+(*          + case a. *)
+(*           * rewrite mult_list_cons_false2''.  *)
+(*             simpl. rewrite IHxs. *)
+(*             rewrite mult_list_cons_false2''. *)
+(*             now rewrite <- add_list_carry_ff_f. *)
+(*           * rewrite mult_list_cons_false1''. *)
+(*             rewrite IHxs. *)
+(*             now rewrite mult_list_cons_false2''. *)
+(*          + case a, b. *)
+(*            * simpl. rewrite IHxs. *)
+(*              now rewrite add_list_carry_ff_f. *)
+(*            * simpl. rewrite IHxs. *)
+(*              now rewrite add_list_carry_ff_f. *)
+(*            * simpl. rewrite IHxs. reflexivity. *)
+(*            * simpl. rewrite IHxs. reflexivity. *)
+(* Qed. *)
+
+(* Lemma mult_list_carry_ff_ff: forall (a b: list bool) n, *)
+(*                        mult_list_carry (false :: a) (false :: b) (S (S n)) = false :: false :: mult_list_carry a b n. *)
+(* Proof. intros a b n. *)
+(*        rewrite mult_list_carry_f_f_1, mult_list_carry_f_f_2. *)
+(*        reflexivity. *)
+(* Qed. *)
+
+(* Lemma mult_list_carry_1: forall (a: list bool), (mult_list_carry a [false; true] 1) = [false]. *)
+(* Proof. intro a. *)
+(*        induction a as [ | a xs IHxs]. *)
+(*        - simpl. reflexivity. *)
+(*        - simpl. case a. *)
+(*          + rewrite mult_list_cons_false2'. *)
+(*            rewrite mult_list_carry_f_f_1. rewrite mult_list_carry_0.  *)
+(*            now unfold add_list. *)
+(*            simpl; lia. *)
+(*          + rewrite mult_list_cons_false2'. *)
+(*            rewrite mult_list_carry_f_f_1. now rewrite mult_list_carry_0. *)
+(*            simpl; lia. *)
+(* Qed. *)
+
+Lemma nsubst_0: forall n, (n - 0)%nat = n.
+Proof. intro n. 
+       induction n as [ | n IHn]; now simpl.
+Qed.
+
+Lemma nsubst_S: forall n, (n <> 0)%nat -> n = S (n - 1)%nat.
+Proof. intro n.
+       induction n as [ | n IHn]; intro H.
+       - now contradict H.
+       - simpl. now rewrite nsubst_0.
+Qed.
+
+
+Lemma not_empty: forall (a: list bool) n, ((length a) > n)%nat -> a <> [].
+Proof. intro a.
+       induction a as [ | a xs IHxs].
+       - intros n H. now contradict H.
+       - intros [ | n] H; easy.
+Qed.
+
+(* Lemma mult_list_carry_add_list_t_f: forall (a b: list bool) n, ((length a) > n)%nat -> *)
+(* (mult_list_carry a (true :: b) (S n)) = (add_list a (false :: mult_list_carry a b n)). *)
+(* Proof. intro a. *)
+(*        induction a as [ | a xs IHxs]. *)
+(*        - intros b n H0. simpl in H0. *)
+(*          now contradict H0. *)
+(*       - intros [ | b ys] n H0. *)
+(*          + case a. *)
+(*            * simpl. *)
+(*              rewrite mult_list_carry_f_f_2. *)
+(*              rewrite add_list_carry_tf_t. *)
+(*              rewrite add_list_carry_tf_t. *)
+(*              apply f_equal. *)
+(*              now rewrite add_list_empty_r, add_list_empty_l. *)
+(*            * rewrite mult_list_carry_f_f_1. *)
+(*              rewrite add_list_carry_ff_f. *)
+(*              apply f_equal. *)
+(*              induction n. *)
+(*                do 2 rewrite mult_list_carry_0. now rewrite add_list_empty_r. *)
+(*                rewrite mult_list_carry_f_f_1. *)
+(*                rewrite <- IHxs. *)
+(*                reflexivity. *)
+(*                simpl in *; lia. *)
+(*          + case a, b. *)
+(*            * simpl. *)
+(*              rewrite mult_list_cons_false2''. *)
+(*              rewrite mult_list_cons_false2''. *)
+(*              rewrite add_list_carry_tf_tf_comm. *)
+(*              symmetry; rewrite add_list_comm; symmetry. *)
+(*              rewrite mult_list_carry_f_f_1. *)
+(*              rewrite add_list_carry_tf_t. *)
+(*              rewrite add_list_carry_ft_t. apply f_equal. *)
+(*              specialize (@IHxs (true :: ys)). *)
+(*              rewrite <- add_list_assoc. *)
+(*              cut ((add_list xs (true :: ys)) = (add_list (true :: ys) xs)). *)
+(*              intro H3. rewrite H3. *)
+(*              rewrite add_list_assoc. *)
+(*              induction n. *)
+(*                do 2 rewrite mult_list_carry_0. now do 3 rewrite add_list_empty_r. *)
+(*              rewrite mult_list_carry_f_f_1. *)
+(*              rewrite IHxs. reflexivity. *)
+(*              simpl in *; lia. *)
+(*              now rewrite add_list_comm. *)
+(*            * simpl. *)
+(*              rewrite mult_list_cons_false2''. *)
+(*              rewrite mult_list_cons_false2''. *)
+(*              rewrite add_list_carry_tf_tf_comm. *)
+(*              symmetry; rewrite add_list_comm; symmetry. *)
+(*              rewrite mult_list_carry_f_f_1. *)
+(*              rewrite add_list_carry_tf_t. *)
+(*              rewrite add_list_carry_ft_t. apply f_equal. *)
+(*              specialize (@IHxs (false :: ys)). *)
+(*              rewrite <- add_list_assoc. *)
+(*              cut ((add_list xs (false :: ys)) = (add_list (false :: ys) xs)). *)
+(*              intro H3. rewrite H3. *)
+(*              rewrite add_list_assoc. *)
+(*              induction n. *)
+(*                do 2 rewrite mult_list_carry_0. now do 3 rewrite add_list_empty_r. *)
+(*              rewrite mult_list_carry_f_f_1. *)
+(*              rewrite IHxs. reflexivity. *)
+(*              simpl in *; lia. *)
+(*              now rewrite add_list_comm. *)
+(*            * rewrite mult_list_carry_f_f_1. *)
+(*              rewrite add_list_carry_ff_f. *)
+(*              apply f_equal. *)
+(*              induction n. *)
+(*                do 2 rewrite mult_list_carry_0. now rewrite add_list_empty_r. *)
+(*              rewrite mult_list_carry_f_f_1. *)
+(*              rewrite IHxs. reflexivity. *)
+(*              simpl in *; lia. *)
+(*            * rewrite mult_list_carry_f_f_1. *)
+(*              rewrite add_list_carry_ff_f. *)
+(*              apply f_equal. *)
+(*              induction n. *)
+(*                do 2 rewrite mult_list_carry_0. now rewrite add_list_empty_r. *)
+(*              rewrite mult_list_carry_f_f_1. *)
+(*              rewrite IHxs. reflexivity. *)
+(*              simpl in *; lia. *)
+(* Qed. *)
+
+(* Lemma mult_list_carry_t_tt_add_list_f_t_tt: forall (a b: list bool) n, ((length a) >= n)%nat -> *)
+(* mult_list_carry (true :: a) (true :: true :: b) (S n) = *)
+(* add_list (false :: a) *)
+(*   (true :: mult_list_carry (true :: a) (true :: b) n). *)
+(* Proof. intros. simpl. *)
+(*         rewrite mult_list_cons_false2''. *)
+(*         rewrite mult_list_cons_false2''. *)
+(*         rewrite add_list_carry_ft_ft_comm. *)
+(*         symmetry; rewrite add_list_comm; symmetry. *)
+(*         rewrite mult_list_carry_f_f_1. *)
+(*         induction n. *)
+(*          do 2 rewrite mult_list_carry_0. rewrite add_list_empty_r. *)
+(*           unfold add_list. simpl. now rewrite add_list_ingr_r. *)
+(*         rewrite mult_list_carry_f_f_1. *)
+(*         rewrite add_list_carry_tf_t. *)
+(*         rewrite add_list_carry_tf_t. apply f_equal. *)
+(*         rewrite add_list_carry_tf_tf_comm. simpl. *)
+(*         rewrite mult_list_carry_add_list_t_f. *)
+(*         rewrite add_list_carry_tf_tf_comm. *)
+(*         rewrite <- add_list_assoc. rewrite <- add_list_assoc. *)
+(*         cut (add_list (true :: b) a = add_list a (true :: b)). *)
+(*         intro H3; now rewrite H3. *)
+(*         now rewrite add_list_comm. *)
+(*         simpl in *; lia. *)
+(* Qed. *)
+
+(* Lemma mult_list_carry_t_tf_add_list_f_t_tf: forall (a b: list bool) n, ((length a) >= n)%nat -> *)
+(* mult_list_carry (true :: a) (true :: false :: b) (S n) = *)
+(* add_list (false :: a) (true :: mult_list_carry (true :: a) (false :: b) n). *)
+(* Proof. intros. simpl. *)
+(*         rewrite mult_list_cons_false2''. *)
+(*         rewrite mult_list_cons_false2''. *)
+(*         rewrite add_list_carry_ft_ft_comm. *)
+(*         symmetry; rewrite add_list_comm; symmetry. *)
+(*         rewrite mult_list_carry_f_f_1. *)
+(*         induction n. *)
+(*          do 2 rewrite mult_list_carry_0. rewrite add_list_empty_r. *)
+(*           unfold add_list. simpl. now rewrite add_list_ingr_r. *)
+(*         rewrite mult_list_carry_f_f_1. *)
+(*         rewrite add_list_carry_tf_t. *)
+(*         rewrite add_list_carry_tf_t. apply f_equal. *)
+(*         rewrite mult_list_carry_add_list_t_f. *)
+(*         rewrite <- add_list_assoc. *)
+(*         rewrite <- add_list_assoc. *)
+(*         cut (add_list (false :: b) a = add_list a (false :: b)). *)
+(*         intro H3; now rewrite H3. *)
+(*         now rewrite add_list_comm. *)
+(*         simpl in *; lia. *)
+(* Qed. *)
+
+(* Lemma mult_list_carry_tt_add_list_ft: forall (a b: list bool) n, ((length a) >= n)%nat -> *)
+(* mult_list_carry a (true :: true :: b) n = *)
+(* add_list a (mult_list_carry a (false :: true :: b) n). *)
+(* Proof. intro a. *)
+(*        induction a as [ | a xs IHxs]. *)
+(*        - intros b n H0. rewrite strictly_positive_0_unique in H0.  *)
+(*            rewrite H0. now do 2 rewrite mult_list_carry_0. *)
+(*        - intros [ | b ys] n H0. *)
+(*          + case a. *)
+(*            * simpl. *)
+(*              induction n. *)
+(*                do 2 rewrite mult_list_carry_0. now rewrite add_list_empty_r. *)
+(*                rewrite mult_list_carry_f_f_2. *)
+(*                rewrite mult_list_carry_f_f_2. *)
+(*                rewrite add_list_carry_tf_t. *)
+(*                rewrite add_list_carry_ff_f. *)
+(*                rewrite add_list_carry_tf_t. apply f_equal. *)
+(*                rewrite IHxs. *)
+(*                rewrite <- add_list_assoc. *)
+(*                rewrite <- add_list_assoc. *)
+(*                cut ((add_list [true] xs) = (add_list xs [true])). now (intro H1; rewrite H1). *)
+(*                now rewrite add_list_comm. *)
+(*                simpl in *; lia. *)
+(*            * simpl. *)
+(*              induction n. *)
+(*                do 2 rewrite mult_list_carry_0. now rewrite add_list_empty_r. *)
+(*                rewrite mult_list_carry_f_f_2. *)
+(*                rewrite mult_list_carry_f_f_2. *)
+(*                rewrite add_list_carry_ff_f. apply f_equal. *)
+(*                rewrite IHxs. reflexivity. *)
+(*                simpl in *; lia. *)
+(*          + case a, b. *)
+(*            * induction n. *)
+(*                do 2 rewrite mult_list_carry_0. now rewrite add_list_empty_r. *)
+(*              rewrite mult_list_carry_t_tt_add_list_f_t_tt. *)
+(*              rewrite mult_list_carry_f_f_2. *)
+(*              rewrite add_list_carry_ft_ft_comm. *)
+(*              now rewrite add_list_comm. *)
+(*              simpl in *; lia. *)
+(*            * induction n. *)
+(*                do 2 rewrite mult_list_carry_0. now rewrite add_list_empty_r. *)
+(*              rewrite mult_list_carry_t_tt_add_list_f_t_tt. *)
+(*              rewrite mult_list_carry_f_f_2. *)
+(*              rewrite add_list_carry_ft_ft_comm. *)
+(*              now rewrite add_list_comm. *)
+(*              simpl in *; lia. *)
+(*            * induction n. *)
+(*                do 2 rewrite mult_list_carry_0. now rewrite add_list_empty_r. *)
+(*              rewrite mult_list_carry_f_f_2. *)
+(*              rewrite mult_list_carry_f_f_1. *)
+(*              rewrite add_list_carry_ff_f. apply f_equal. *)
+(*              rewrite IHxs. *)
+(*              rewrite mult_list_cons_false1''. reflexivity. *)
+(*              simpl in *; lia. *)
+(*            * induction n. *)
+(*                do 2 rewrite mult_list_carry_0. now rewrite add_list_empty_r. *)
+(*              rewrite mult_list_carry_f_f_2. *)
+(*              rewrite mult_list_carry_f_f_1. *)
+(*              rewrite add_list_carry_ff_f. apply f_equal. *)
+(*              rewrite IHxs. *)
+(*              rewrite mult_list_cons_false1''. reflexivity. *)
+(*              simpl in *; lia. *)
+(* Qed. *)
+
+(* Lemma mult_list_carry_tf_add_list_ff: forall (a b: list bool) n, ((length a) >= n)%nat  -> *)
+(* mult_list_carry a (true :: false :: b) n = *)
+(* add_list a (mult_list_carry (false :: a) (false :: b) n). *)
+(* Proof. intro a. *)
+(*        induction a as [ | a xs IHxs]. *)
+(*        - intros b n H0. rewrite strictly_positive_0_unique in H0.  *)
+(*            rewrite H0. now do 2 rewrite mult_list_carry_0. *)
+(*        - intros [ | b ys] n H0. *)
+(*          + case a. *)
+(*            * simpl. *)
+(*              induction n. *)
+(*                do 2 rewrite mult_list_carry_0. now rewrite add_list_empty_r. *)
+(*                rewrite mult_list_carry_f_f_2. *)
+(*                rewrite mult_list_carry_f_f_2. *)
+(*                rewrite add_list_carry_tf_t. *)
+(*                rewrite add_list_carry_ff_f. *)
+(*                rewrite add_list_carry_tf_t. apply f_equal. *)
+(*                rewrite IHxs. *)
+(*                rewrite <- add_list_assoc. *)
+(*                rewrite <- add_list_assoc. *)
+(*                cut ((add_list [false] xs) = (add_list xs [false])). now (intro H1; rewrite H1). *)
+(*                now rewrite add_list_comm. *)
+(*                simpl in *; lia. *)
+(*            * simpl. *)
+(*              induction n. *)
+(*                do 2 rewrite mult_list_carry_0. now rewrite add_list_empty_r. *)
+(*                rewrite mult_list_carry_f_f_2. *)
+(*                rewrite mult_list_carry_f_f_2. *)
+(*                rewrite add_list_carry_ff_f. apply f_equal. *)
+(*                rewrite IHxs. reflexivity. *)
+(*                simpl in *; lia. *)
+(*          + case a, b. *)
+(*            * induction n. *)
+(*                do 2 rewrite mult_list_carry_0. now rewrite add_list_empty_r. *)
+(*              rewrite mult_list_carry_t_tf_add_list_f_t_tf. *)
+(*              rewrite mult_list_carry_f_f_2. *)
+(*              rewrite add_list_carry_ft_ft_comm. *)
+(*              now rewrite add_list_comm. *)
+(*              simpl in *; lia. *)
+(*            * induction n. *)
+(*                do 2 rewrite mult_list_carry_0. now rewrite add_list_empty_r. *)
+(*              rewrite mult_list_carry_t_tf_add_list_f_t_tf. *)
+(*              rewrite mult_list_carry_f_f_2. *)
+(*              rewrite add_list_carry_ft_ft_comm. *)
+(*              now rewrite add_list_comm. *)
+(*              simpl in *; lia. *)
+(*            * induction n. *)
+(*                do 2 rewrite mult_list_carry_0. now rewrite add_list_empty_r. *)
+(*              rewrite mult_list_carry_f_f_2. *)
+(*              rewrite mult_list_carry_f_f_1. *)
+(*              rewrite add_list_carry_ff_f. apply f_equal. *)
+(*              rewrite IHxs. *)
+(*              rewrite mult_list_cons_false1''. reflexivity. *)
+(*              simpl in *; lia. *)
+(*            * induction n. *)
+(*                do 2 rewrite mult_list_carry_0. now rewrite add_list_empty_r. *)
+(*              rewrite mult_list_carry_f_f_2. *)
+(*              rewrite mult_list_carry_f_f_1. *)
+(*              rewrite add_list_carry_ff_f. apply f_equal. *)
+(*              rewrite IHxs. *)
+(*              rewrite mult_list_cons_false1''. reflexivity. *)
+(*              simpl in *; lia. *)
+(* Qed. *)
+
+(* Lemma mult_list_carry_ft_add_list_f_ff: forall (a b: list bool) n, ((length a) >= n)%nat -> *)
+(* (mult_list_carry a (false :: true :: b) n) = *)
+(* (add_list (false :: a) ((mult_list_carry a (false :: false :: b) n))). *)
+(* Proof. intro a. *)
+(*        induction a as [ | a xs IHxs]. *)
+(*        - intros b n H0. rewrite strictly_positive_0_unique in H0.  *)
+(*            rewrite H0. now do 2 rewrite mult_list_carry_0. *)
+(*        - intros [ | b ys] n H0. *)
+(*          + case a. *)
+(*            * simpl. *)
+(*              induction n. *)
+(*                do 2 rewrite mult_list_carry_0. now rewrite add_list_empty_r. *)
+(*                rewrite mult_list_carry_f_f_2. *)
+(*                rewrite mult_list_carry_f_f_2. *)
+(*                rewrite add_list_carry_ff_f. *)
+(*                rewrite add_list_carry_ff_f. *)
+(*                rewrite add_list_carry_ff_f. apply f_equal. *)
+(*                rewrite IHxs. *)
+(*                rewrite <- add_list_assoc. *)
+(*                rewrite <- add_list_assoc. *)
+(*                cut ((add_list [true] (false :: xs)) = (add_list (true :: xs) [false])). now (intro H1; rewrite H1). *)
+(*                now rewrite add_list_comm. *)
+(*                simpl in *; lia. *)
+(*            * simpl. *)
+(*              induction n. *)
+(*                do 2 rewrite mult_list_carry_0. now rewrite add_list_empty_r. *)
+(*                rewrite mult_list_carry_f_f_2. *)
+(*                rewrite mult_list_carry_f_f_2. *)
+(*                rewrite add_list_carry_ff_f. apply f_equal. *)
+(*                rewrite IHxs. reflexivity. *)
+(*                simpl in *; lia. *)
+(*          + case a, b. *)
+(*            * induction n. *)
+(*                do 2 rewrite mult_list_carry_0. now rewrite add_list_empty_r. *)
+(*              rewrite mult_list_carry_f_f_2. *)
+(*              rewrite mult_list_carry_f_f_2. *)
+(*              rewrite add_list_carry_ff_f. apply f_equal. *)
+(*              induction n. *)
+(*                do 2 rewrite mult_list_carry_0. now rewrite add_list_empty_r. *)
+(*                rewrite mult_list_carry_t_tt_add_list_f_t_tt. *)
+(*                rewrite mult_list_carry_f_f_2. *)
+(*              rewrite add_list_carry_ft_ft_comm. *)
+(*              now rewrite add_list_comm. *)
+(*              simpl in *; lia. *)
+(*            * induction n. *)
+(*                do 2 rewrite mult_list_carry_0. now rewrite add_list_empty_r. *)
+(*              rewrite mult_list_carry_f_f_2. *)
+(*              rewrite mult_list_carry_f_f_2. *)
+(*              rewrite add_list_carry_ff_f. apply f_equal. *)
+(*              induction n. *)
+(*                do 2 rewrite mult_list_carry_0. now rewrite add_list_empty_r. *)
+(*              rewrite mult_list_carry_t_tf_add_list_f_t_tf. *)
+(*              rewrite mult_list_carry_f_f_2. *)
+(*              rewrite add_list_carry_ft_ft_comm. *)
+(*              now rewrite add_list_comm. *)
+(*              simpl in *; lia. *)
+(*            * induction n. *)
+(*                do 2 rewrite mult_list_carry_0. now rewrite add_list_empty_r. *)
+(*              rewrite mult_list_carry_f_f_2. *)
+(*              rewrite mult_list_carry_f_f_2. *)
+(*              rewrite add_list_carry_ff_f. apply f_equal. *)
+(*              induction n. *)
+(*                do 2 rewrite mult_list_carry_0. now rewrite add_list_empty_r. *)
+(*              rewrite mult_list_carry_tt_add_list_ft. reflexivity. *)
+(*              simpl in *; lia. *)
+(*            * induction n. *)
+(*                do 2 rewrite mult_list_carry_0. now rewrite add_list_empty_r. *)
+(*              rewrite mult_list_carry_f_f_2. *)
+(*              rewrite mult_list_carry_f_f_2. *)
+(*              rewrite add_list_carry_ff_f. apply f_equal. *)
+(*              induction n. *)
+(*                do 2 rewrite mult_list_carry_0. now rewrite add_list_empty_r. *)
+(*                rewrite mult_list_carry_tf_add_list_ff. reflexivity. *)
+(*              simpl in *; lia. *)
+(* Qed. *)
+
+(* Lemma mult_list_carry_comm: forall (a b: list bool) n, ((length a) >= n)%nat -> ((length b) >= n)%nat -> *)
+(*                             mult_list_carry a b n = mult_list_carry b a n. *)
+(* Proof. intro a. *)
+(*        induction a as [ | a xs IHxs]. *)
+(*        - intros b n H0 H1. rewrite strictly_positive_0_unique in H0. rewrite H0. *)
+(*          do 2 rewrite mult_list_carry_0. reflexivity. *)
+(*        - intros [ | b ys] n H0 H1. *)
+(*          + rewrite strictly_positive_0_unique in H1. rewrite H1. *)
+(*            do 2 rewrite mult_list_carry_0. reflexivity. *)
+(*          + case a, b. *)
+(*            * simpl. *)
+(*              induction n. *)
+(*              do 2 rewrite mult_list_carry_0. now rewrite add_list_empty_r. *)
+(*              rewrite mult_list_carry_f_f_2. *)
+(*              rewrite mult_list_carry_f_f_2. *)
+(*              rewrite add_list_carry_tf_t. *)
+(*              rewrite add_list_carry_tf_t. apply f_equal. *)
+(*              induction n. *)
+(*                do 2 rewrite mult_list_carry_0.  *)
+(*                now do 2 rewrite add_list_empty_r. *)
+(*              rewrite mult_list_carry_add_list_t_f. *)
+(*              rewrite mult_list_carry_add_list_t_f. *)
+(*              rewrite IHxs. *)
+(*              rewrite <- add_list_assoc. *)
+(*              rewrite <- add_list_assoc. *)
+(*              cut (add_list xs ys = add_list ys xs). now (intro H2 ;rewrite H2). *)
+(*              now rewrite add_list_comm. *)
+(*              simpl in *; lia. *)
+(*              simpl in *; lia. *)
+(*              simpl in *; lia. *)
+(*              simpl in *; lia. *)
+(*            * simpl. *)
+(*              induction n. *)
+(*                do 2 rewrite mult_list_carry_0. now rewrite add_list_empty_r. *)
+(*                rewrite mult_list_carry_f_f_2. *)
+(*                rewrite mult_list_carry_f_f_2. *)
+(*                rewrite add_list_carry_ff_f. apply f_equal. *)
+(*              induction n. *)
+(*                do 2 rewrite mult_list_carry_0.  *)
+(*                now rewrite add_list_empty_r. *)
+(*              rewrite mult_list_carry_add_list_t_f. *)
+(*              rewrite mult_list_carry_f_f_2. *)
+(*              rewrite IHxs. reflexivity. *)
+(*              simpl in *; lia. *)
+(*              simpl in *; lia. *)
+(*              simpl in *; lia. *)
+(*            * simpl. *)
+(*              induction n. *)
+(*                do 2 rewrite mult_list_carry_0. now rewrite add_list_empty_r. *)
+(*                rewrite mult_list_carry_f_f_2. *)
+(*                rewrite mult_list_carry_f_f_2. *)
+(*                rewrite add_list_carry_ff_f. apply f_equal. *)
+(*              induction n. *)
+(*                do 2 rewrite mult_list_carry_0.  *)
+(*                now rewrite add_list_empty_r. *)
+(*              rewrite mult_list_carry_add_list_t_f. *)
+(*              rewrite mult_list_carry_f_f_2. *)
+(*              rewrite IHxs. reflexivity. *)
+(*              simpl in *; lia. *)
+(*              simpl in *; lia. *)
+(*              simpl in *; lia. *)
+(*            * simpl. *)
+(*              induction n. *)
+(*                now do 2 rewrite mult_list_carry_0. *)
+(*                rewrite mult_list_carry_f_f_2. *)
+(*                rewrite mult_list_carry_f_f_2. apply f_equal. *)
+(*              induction n. *)
+(*                now do 2 rewrite mult_list_carry_0.  *)
+(*              rewrite mult_list_carry_f_f_2. *)
+(*              rewrite mult_list_carry_f_f_2. apply f_equal. *)
+(*              rewrite IHxs. reflexivity. *)
+(*              simpl in *; lia. *)
+(*              simpl in *; lia. *)
+(* Qed. *)
+
+(* Lemma mult_list_comm: forall (a b: list bool) n, n = (length a) -> (n = length b) -> (mult_list a b) = (mult_list b a). *)
+(* Proof. intros a b n H0 H1. *)
+(*        unfold mult_list.  *)
+(*        rewrite <- H0, H1. *)
+(*        apply mult_list_carry_comm; lia. *)
+(* Qed. *)
+
+(* (* bitvector MULT properties *) *)
+
+Lemma prop_mult_bool_step_k_h_len: forall a b c k,
+length (mult_bool_step_k_h a b c k) = length a.
+Proof. intro a.
+       induction a as [ | xa xsa IHa ].
+       - intros. simpl. easy.
+       - intros.
+         case b in *. simpl. rewrite IHa. simpl. omega.
+         simpl. case (k - 1 <? 0)%Z; simpl; now rewrite IHa.
+Qed. 
+
+
+Lemma empty_list_length: forall {A: Type} (a: list A), (length a = 0)%nat <-> a = [].
+Proof. intros A a.
+       induction a; split; intros; auto; contradict H; easy.
+Qed.
+
+Lemma prop_mult_bool_step: forall k' a b res k, 
+                       length (mult_bool_step a b res k k') = (length res)%nat.
+Proof. intro k'.
+       induction k'.
+       - intros. simpl. rewrite prop_mult_bool_step_k_h_len. simpl. omega.
+       - intros. simpl. rewrite IHk'. rewrite prop_mult_bool_step_k_h_len. simpl; omega.
+Qed.
+
+Lemma and_with_bool_len: forall a b, length (and_with_bool a (nth 0 b false)) = length a.
+Proof. intro a.
+       - induction a.
+         intros. now simpl.
+         intros. simpl. now rewrite IHa.
+Qed.
+
+
+Lemma bv_mult_size a b: size (bv_mult a b) = _size.
+Admitted.
+(*
+Proof. unfold size, bv_mult, bits, mult_list.
+       case_eq (size a =? size b).
+       - intros. now unfold size in *.
+       - intros. unfold size in *. contradict H.
+         rewrite N.eqb_compare, N.compare_refl. easy.
+Qed.
+*)
+ 
+				     
+(* Proof. *)
+(*   unfold size_bv_mult, bv_mult. *)
+(*   case_eq (size a =? size b); intros. *)
+(*   - rewrite N.eqb_eq in H. unfold size in *. *)
+(*     apply f_equal. unfold bits. *)
+(*     symmetry; apply mult_list_length_eq. *)
+(*     now apply Nat2N.inj in H. *)
+(*   - now unfold size in *. *)
+(* Qed. *)
+
+(* Lemma bv_mult_comm: forall n a b, (size a) = n -> (size b) = n -> bv_mult a b = bv_mult b a. *)
+(* Proof. intros n a b H0 H1. *)
+(*        unfold bv_mult, size, bits in *. rewrite H0, H1. *)
+(*        rewrite N.eqb_compare. rewrite N.compare_refl. *)
+(*        rewrite (@mult_list_comm a b (nat_of_N n)). reflexivity. *)
+(*        rewrite <- H0. now rewrite Nat2N.id. *)
+(*        rewrite <- H1. now rewrite Nat2N.id. *)
+(* Qed. *)
+
+End RAWBITVECTOR_LIST_FIXED.
+
+Module BITVECTOR_LIST_FIXED <: BITVECTOR_FIXED := RAW2BITVECTOR_FIXED(RAWBITVECTOR_LIST_FIXED).
+
+
+
+(************************************************************************************************************)
 
 Module RAWBITVECTOR_LIST <: RAWBITVECTOR.
 
@@ -519,7 +2992,7 @@ Fixpoint mult_bool_step_k_h (a b: list bool) (c: bool) (k: Z) : list bool :=
 
 
 Fixpoint top_k_bools (a: list bool) (k: int) : list bool :=
-  if (k == 0)%int then nil
+  if (k == 0)%int63 then nil
   else match a with
          | nil => nil
          | ai :: a' => ai :: top_k_bools a' (k - 1)
